Progress towards generalization and tseitin

src/basic.lean
@@ -9,13 +9,20 @@
 
 import data.bool
 import data.list.basic
+import data.list.nodup
+import init.data.nat.lemmas
+import tactic
+
+import init.function
 
 open list
+open function
+
+universes u v
+variables {α : Type u} {β : Type v}
 
 -- Define shorthand for XOR
 notation a ⊕ b := bxor a b
---notation a ∨ b := bor a b
---notation a ∧ b := band a b
 
 -- Some trivial, useful theorems
 @[simp] theorem bxor_tt_left  : ∀ a, bxor tt a = bnot a := dec_trivial
@@ -23,6 +30,31 @@ notation a ⊕ b := bxor a b
 
 @[simp] theorem cond_tt_ff : ∀ a, cond a tt ff = a := dec_trivial
 @[simp] theorem cond_ff_tt : ∀ a, cond a ff tt = bnot a := dec_trivial
+
+-- I feel like this exists in the library somewhere...
+theorem tt_of_cond_eq_tt_of_ne [decidable_eq α] {c d : α} {b : bool} : 
+  c ≠ d → cond b c d = c → b = tt :=
+begin
+  cases b,
+  { simp, intros h₁ h₂, exact absurd h₂.symm h₁ },
+  { simp }
+end
+
+theorem ff_of_cond_eq_ff_of_ne [decidable_eq α] {c d : α} {b : bool} :
+  c ≠ d → cond b c d = d → b = ff :=
+begin
+  cases b,
+  { simp },
+  { simp,
+    intros h₁ h₂,
+    exact absurd h₂ h₁ }
+end
+
+theorem band_tt_of_and_tt {b₁ b₂ : bool} : b₁ = tt ∧ b₂ = tt → b₁ && b₂ = tt :=
+begin
+  rintros ⟨h₁, h₂⟩,
+  simp [h₁, h₂]
+end
 
 -- Expand xor in terms of other boolean operations
 -- (Proof seems inane - shorten?)
@@ -43,55 +75,44 @@ begin
   intros ha hb, simp [ha, hb]
 end
 
-theorem bool_by_cases : ∀ (b : bool), b = tt ∨ b = ff
-| tt := by { left, refl }
-| ff := by { right, refl }
-
 /- This is a shorthand for absurd that derives from a boolean that is true and false -/
 theorem absurd_bool {a : bool} {b : Prop} : a = tt → a = ff → b :=
 assume h₁ h₂, absurd h₁ (neq_of_ff_of_tt rfl h₂).symm
 
 /- Reasoning about cond is helpful if the result of the cond is known -/
-theorem cond_tt_of_cond_eq_first_of_ne {α : Type} [decidable_eq α] {a₁ a₂ : α} {b : bool} : 
-  a₁ ≠ a₂ → cond b a₁ a₂ = a₁ → b = tt :=
-begin
-  intros hne hcond,
-  rcases bool_by_cases b,
-  { exact h },
-  { simp [h] at hcond, exact absurd hcond (ne.symm hne) }
-end
+theorem cond_tt_of_cond_eq_first_of_ne [decidable_eq α] {a₁ a₂ : α} (b : bool) : 
+  a₂ ≠ a₂ → cond b a₁ a₂ = a₁ → b = tt :=
+by cases b; simp [imp_false]
 
-theorem cond_ff_of_cond_eq_second_of_ne {α : Type} [decidable_eq α] {a₁ a₂ : α} {b : bool} :
+theorem cond_ff_of_cond_eq_second_of_ne [decidable_eq α] {a₁ a₂ : α} (b : bool) :
   a₁ ≠ a₂ → cond b a₁ a₂ = a₂ → b = ff :=
-begin
-  intros hne hcond,
-  rcases bool_by_cases b,
-  { simp [h] at hcond, exact absurd hcond hne },
-  { exact h }
-end
+by cases b; simp [imp_false]
 
-theorem list_by_cases {α : Type} : ∀ (l : list α), l = [] ∨ ∃ b L, l = b :: L
-| []        := by { left, refl }
-| (x :: xs) := by { right, use [x, xs] }
+theorem cond_tt_of_not_cond_eq_second_of_ne [decidable_eq α] {a₁ a₂ : α} (b : bool) :
+  a₁ ≠ a₂ → ¬(cond b a₁ a₂ = a₂) → b = tt :=
+by cases b; simp
 
-theorem ne_tail_of_eq_head_of_ne {α : Type} [decidable_eq α] {a b : α} : ∀ {l₁ : list α},
+theorem cond_ff_of_not_cond_eq_first_of_ne [decidable_eq α] {a₁ a₂ : α} (b : bool) :
+  a₂ ≠ a₁ → ¬(cond b a₁ a₂ = a₁) → b = ff :=
+by cases b; simp
+
+theorem ne_tail_of_eq_head_of_ne [decidable_eq α] {a b : α} : ∀ {l₁ : list α},
   ∀ {l₂ : list α}, (a :: l₁) ≠ (b :: l₂) → a = b → l₁ ≠ l₂
 | []        := by simp
 | (x :: xs) := begin
   intros l₂ hneq heq,
   by_contradiction,
-  simp at h,
   exact absurd (congr (congr_arg cons heq) h) hneq
 end
 
 -- Some facts about map that help
-theorem exists_of_map_singleton {α β : Type} {f : α → β} {b : β} :
+theorem exists_of_map_singleton {f : α → β} {b : β} :
   ∀ {l : list α}, map f l = [b] → ∃ a, [a] = l ∧ f a = b
 | []        := by { contradiction }
 | [x]       := by { simp [map_cons] }
 | (x :: y :: ys) := by { simp }
 
-theorem exists_cons_of_map_cons {α β : Type} {f : α → β} {b : β} {bs : list β} :
+theorem exists_cons_of_map_cons {f : α → β} {b : β} {bs : list β} :
   ∀ {l : list α}, map f l = b :: bs → ∃ h L, l = h :: L ∧ f h = b ∧ map f L = bs
 | []        := by { contradiction }
 | (x :: xs) := begin 
@@ -101,7 +122,7 @@ theorem exists_cons_of_map_cons {α β : Type} {f : α → β} {b : β} {bs : li
 end
 
 -- If instead the list from above is a map construction too
-theorem exists_map_cons_of_map_cons {α β : Type} {f : α → β} {a : α} {as : list α} :
+theorem exists_map_cons_of_map_cons {f : α → β} {a : α} {as : list α} :
   ∀ {l : list α}, map f l = map f (a :: as) → ∃ h L, l = h :: L ∧ f h = f a ∧ map f L = map f as
 | []        := by { contradiction }
 | (x :: xs) := begin
@@ -110,8 +131,12 @@ theorem exists_map_cons_of_map_cons {α β : Type} {f : α → β} {a : α} {as 
   use [x, xs], simp [hx, hxs]
 end
 
+theorem mem_map_append {l₁ l₂ : list α} {f : α → β} {b : β} :
+  b ∈ map f (l₁ ++ l₂) → b ∈ map f l₁ ∨ b ∈ map f l₂ :=
+by simp
+
 -- Or facts about filter
-theorem length_filter {α : Type} {p : α → Prop} [decidable_pred p] {l : list α} : 
+theorem length_filter {p : α → Prop} [decidable_pred p] {l : list α} : 
   length (filter p l) ≤ length l :=
 begin
   induction l with x xs ih,
@@ -119,4 +144,156 @@ begin
   { by_cases p x,
     { simp [filter_cons_of_pos _ h, ih] },
     { simp [filter_cons_of_neg _ h, ih, le_add_right] } }
+end
+
+-- Sublists need membership theorems, too
+theorem mem_of_mem_sublist {l₁ l₂ : list α} {a : α} :
+  a ∈ l₁ → l₁ <+ l₂ → a ∈ l₂ :=
+assume ha hl, sublist.subset hl ha
+
+theorem not_mem_of_sublist_of_not_mem {l₁ l₂ : list α} {a : α} :
+  a ∉ l₂ → l₁ <+ l₂ → a ∉ l₁ :=
+assume ha hl h, absurd ((sublist.subset hl) h) ha
+
+-- Very sad theorems on nats
+def max_nat : list nat → nat
+| []        := 0
+| (n :: ns) := max n (max_nat ns)
+
+theorem max_nat_is_max (l : list nat) : ∀ (n : nat), n ∈ l → n ≤ max_nat l :=
+begin
+  induction l with m ms ih,
+  { simp },
+  { intros n hn,
+    rcases eq_or_mem_of_mem_cons hn with rfl | hms,
+    { simp [max_nat] },
+    { simp [ih n hms, max_nat] } }
+end
+
+theorem not_mem_of_gt_max_nat {l : list nat} {n : nat} : n > max_nat l → n ∉ l :=
+begin
+  contrapose, simp, exact max_nat_is_max l n
+end
+
+theorem not_mem_of_gt_max {l : list nat} {n : nat} : n > foldr max 0 l → n ∉ l :=
+begin
+  induction l with m ms ih,
+  { simp },
+  { simp,
+    intros hm hn,
+    exact not_or_distrib.mpr (and.intro (ne_of_gt hm) (ih hn)) }
+end
+
+theorem exists_not_mem_of_gt_max {f : α → nat} (hf : bijective f) {l : list α} :
+  ∀ {n : nat}, n > foldr max 0 (map f l) → ∃ (a : α), f a = n ∧ a ∉ l :=
+begin
+  intros n hn,
+  rcases (bijective_iff_exists_unique f).mp hf n with ⟨b, hb, _⟩,
+  use b,
+  split,
+  { simp [hb] },
+  { have := not_mem_of_gt_max hn,
+    revert this,
+    contrapose,
+    simp,
+    intro h,
+    use [b, h, hb] }
+end
+
+-- A simple nat result - can be tightened up, but how?
+theorem ne_of_add_eq_of_gt_zero {a b c : nat} : a > 0 → a + b = c → b ≠ c :=
+begin
+  intros ha habc hbc,
+  rw hbc at habc,
+  have : a + c > c, from lt_add_of_pos_left c ha,
+  rw habc at this,
+  exact nat.lt_asymm this this,
+end
+
+-- Maximum values that map to general α
+theorem infimum_gt_list {f : nat → α} (f_inj : injective f) (l : list α) :
+  ∃ (n : nat), ∀ (m : nat), m ≥ n → f m ∉ l :=
+begin
+  induction l with a as ih,
+  { simp [not_mem_nil] },
+  { rcases ih with ⟨n, hn⟩,
+    by_cases h : ∃ (b : nat), f b = a,
+    { rcases h with ⟨b, hb⟩,
+      by_cases hnb : n > b,
+      { use n, 
+        intros m hm,
+        apply not_mem_cons_of_ne_of_not_mem,
+        { rw ← hb,
+          exact (injective.ne_iff f_inj).mpr (ne_of_gt (gt_of_ge_of_gt hm hnb)) },
+        { exact hn m hm } },
+      { use b + 1,
+        intros m hm,
+        simp at hnb,
+        apply not_mem_cons_of_ne_of_not_mem,
+        { rw ← hb,
+          exact (injective.ne_iff f_inj).mpr (ne_of_gt (nat.succ_le_iff.mp hm)) },
+        { exact hn m (le_trans hnb (nat.le_of_succ_le hm)) } } },
+    { simp at h,
+      use n,
+      intros m hm,
+      apply not_mem_cons_of_ne_of_not_mem,
+      { exact h m },
+      { exact hn m hm } } }
+end
+
+/-
+def infimum_of_bijective {f : nat → α} (f_bij : bijective f) : list α → α
+| []:= f 0
+| l := max_nat (map (λ a, ))
+-/
+
+@[simp] theorem nil_inter [decidable_eq α] (l : list α) : l ∩ [] = [] :=
+eq_nil_of_subset_nil (inter_subset_right l [])
+
+theorem zero_left_of_add_zero {n m : nat} : 0 = n + m → n = 0 :=
+begin
+  cases m,
+  { rw add_zero n, intro h, exact h.symm },
+  { intro h, linarith }
+end
+
+theorem zero_right_of_add_zero {n m : nat} : 0 = n + m → m = 0 :=
+begin
+  cases n,
+  { rw zero_add m, intro h, exact h.symm },
+  { intro h, linarith }
+end
+
+theorem mem_fst_map_of_mem {l : list (α × β)} {a : α} {b : β} :
+  (a, b) ∈ l → a ∈ map prod.fst l :=
+begin
+  intro h,
+  apply mem_map.mpr,
+  use [(a, b), h]
+end
+
+theorem mem_snd_map_of_mem {l : list (α × β)} {a : α} {b : β} :
+  (a, b) ∈ l → b ∈ map prod.snd l :=
+begin
+  intro h,
+  apply mem_map.mpr,
+  use [(a, b), h]
+end
+
+theorem length_lt_length_cons (a : α) (l : list α) :
+  length l < length (a :: l) :=
+by simp [length]
+
+theorem strong_induction_on_lists [inhabited α] {p : list α → Prop} (l : list α)
+  (h : ∀ l₁, (∀ l₂, length l₂ < length l₁ → p l₂) → p l₁) : p l :=
+suffices ∀ (l₁ : list α) (l₂ : list α), length l₂ < length l₁ → p l₂,
+  from this ((arbitrary α) :: l) l (length_lt_length_cons (arbitrary α) l),
+begin
+  intro l₁, induction l₁ with a as ih,
+  { intros l₂ h₁, unfold length at h₁, exact absurd h₁ (l₂.length).not_lt_zero },
+  { intros m h₁,
+    unfold length at h₁,
+    apply or.by_cases (decidable.lt_or_eq_of_le (nat.le_of_lt_succ h₁)),
+    { intros, apply ih, assumption },
+    { intro hlen, have := h m, rw hlen at this, exact this ih } }
 end
