src/xor/tseitin.lean
@@ -5,13 +5,19 @@ Authors: Cayden Codel, Jeremy Avidgad, Marijn Heule
 Carnegie Mellon University
 -/
 
-import cnf.literal
-import cnf.clause
-import cnf.cnf
-import xor.xor
+import cnf.literal_general
+import cnf.clause_general
+import cnf.cnf_general
+import xor.xor_general
+import cnf.gensym
 
 import data.list.basic
-import data.list.min_max
+import data.nat.basic
+import init.function
+
+universe u
+
+variables {V : Type u} [inhabited V] [decidable_eq V]
 
 open literal
 open clause
@@ -19,10 +25,13 @@ open cnf
 open xor_gate
 
 open list
+open assignment
+open function
 
 namespace tseitin_xor
 
-lemma dropn_len {α : Type} {n : nat} {a : α} {l : list α} : n > 1 → length l > n → length (l.drop n ++ [a]) < length l :=
+lemma dropn_len {α : Type u} {n : nat} (a : α) {l : list α} :
+  n > 1 → length l > n → length (l.drop n ++ [a]) < length l :=
 begin
   intros hn hl,
   induction l with x xs ih,
@@ -31,14 +40,210 @@ begin
     { simp [h, gt.lt hn] },
     { simp at hl,
       have red := ih (gt.lt (array.push_back_idx hl (ne.symm h))), -- strange theorem
-      simp [nat.sub_add_eq_add_sub (nat.lt_succ_iff.mp hl)] at red,
+      simp at red,
+      simp [tsub_add_eq_add_tsub (nat.lt_succ_iff.mp hl)] at red,
       simp [red] } }
+end
+
+lemma three_gt_one : 3 > 1 :=
+nat.one_lt_succ_succ 1
+
+def thelper : list (literal V) → gensym V → cnf V
+| [] g₁ := [[]]
+| l  g₁ := if h : length l ≤ 3 then xor_cnf l else
+                  let ⟨v, g₂⟩ := gensym.fresh g₁ in
+                  have length (l.drop 3 ++ [Pos v]) < length l,
+                    from (dropn_len _ three_gt_one (not_le.mp h)),
+                  xor_cnf (l.take 3 ++ [Neg v]) ++ thelper (l.drop 3 ++ [Pos v]) g₂
+using_well_founded {
+  rel_tac := λ a b, `[exact ⟨_, measure_wf (λ σ, list.length σ.1)⟩],
+  dec_tac := tactic.assumption
+}
+
+def tseitin_xor3 {f : nat → V} (hf : injective f) {g : V → nat} (hg : injective g)
+  (hfg : right_inverse f g) (l : list (literal V)) : cnf V :=
+thelper l (gensym.seed hf hg hfg (clause.vars l))
+
+lemma exists_tseitin_of_xor_cnf {f : nat → V} (hf : injective f)
+  {g : V → nat} (hg : injective g) (hfg : right_inverse f g) 
+  {l : list (literal V)} :
+  (∃ (α : assignment V), cnf.eval α (tseitin_xor3 hf hg hfg l) = tt) → 
+   ∃ (α₂ : assignment V), cnf.eval α₂ (xor_cnf l) = tt :=
+begin
+  rintros ⟨α, ha⟩,
+  
+end
+
+
+lemma exists_xor_cnf_of_tseitin {f : nat → V} (hf : injective f)
+  {g : V → nat} (hg : injective g) (hfg : right_inverse f g) 
+  {l : list (literal V)} :
+  (∃ (α : assignment V), cnf.eval α (xor_cnf l) = tt) → 
+   ∃ (α₂ : assignment V), cnf.eval α₂ (tseitin_xor3 hf hg hfg l) = tt :=
+begin
+
+end
+
+
+noncomputable def tseitin_xor3 {f : V → nat} (hf : bijective f) : list (literal V) → list V → cnf V
+| [] _ := [[]]
+| l vs := if h : length l ≤ 3 then xor_cnf l else
+    have exi : ∃ (v : V), v ∉ vs, from exists_not_mem_of_bijection hf vs,
+    have length (l.drop 3 ++ [Pos (classical.some exi)]) < length l,
+      from (dropn_len _ three_gt_one (not_le.mp h)),
+    xor_cnf (l.take 3 ++ [Neg (classical.some exi)]) ++ 
+      (tseitin_xor3 (l.drop 3 ++ [Pos (classical.some exi)]) ((classical.some exi) :: vs))
+using_well_founded {
+  rel_tac := λ a b, `[exact ⟨_, measure_wf (λ σ, list.length σ.1)⟩],
+  dec_tac := tactic.assumption
+}
+/-
+(∃ (α : assignment V), cnf.eval α (xor_cnf l) = tt) →
+  ∃ (α₂ : assignment V), eval α₂ l = tt :=
+-/
+
+/-
+/-
+It is noncomputable because pulling a variable from the witness in an exists hypothesis
+is not non-classical. In the future, attempt to use gensym in place of the ∃hyp.
+-/
+
+
+lemma empty_intersect_of_empty_intersect {l : list (literal V)} {g : gensym V} :
+  ∀ (l₂ : list (literal V)), l₂ ⊆ l → (∀ (n : nat), clause.vars l ∩ (g.nfresh n).1 = []) →
+  ∀ (m : nat), clause.vars l₂ ++ [g.fresh.1] ∩ (g.fresh.2.nfresh m).1 = [] :=
+begin
+  induction l with l ls ih,
+  { intros l₂ hl₂ hn m,
+    have := eq_nil_of_subset_nil hl₂,
+    rw this,
+    simp,
+    cases m,
+    { simp [gensym.nfresh] },
+    {
+      
+    }
+  }
+end
+
+def tx3 : Π (l : list (literal V)), Π (g : gensym V),
+          (∀ n : nat, clause.vars l ∩ (g.nfresh n).1 = []) → cnf V
+| l g p := if h : length l ≤ 3 then xor_cnf l else
+          let ⟨v, g₂⟩ := gensym.fresh g in
+          xor_cnf (l.take 3 ++ [Neg v]) ++ (tx3 (l.drop 3 ++ [Pos v]) g₂ p)
+
+/-
+def tx3_helper : list (literal V) × gensym (literal V) → cnf V 
+| ⟨[], _⟩ := [[]]
+| ⟨l, g⟩  := if h : length l ≤ 3 then xor_cnf l else
+    let ⟨v, g2⟩ := gensym.fresh g in
+    have length (l.drop 3 ++ [set_pos v]) < length l,
+      from (dropn_len _ three_gt_one (not_le.mp h)),
+    xor_cnf (l.take 3 ++ [set_neg v]) ++ (tx3_helper ⟨(l.drop 3 ++ [set_pos v]), g2⟩)
+using_well_founded {
+  rel_tac := λ a b, `[exact ⟨_, measure_wf (λ σ, list.length σ.1)⟩],
+  dec_tac := tactic.assumption
+}
+
+def tx3 {f : nat → (literal V)} (hf : injective f) (n : nat) : cnf V :=
+  tx3_helper (gensym.nfresh (gensym.init hf) n)
+
+lemma tx3_base_case {f : nat → (literal V)} (hf : injective f) {n : nat} :
+  n ≤ 3 → cnf.equisatisfiable (tx3 hf n) (xor_cnf (gensym.nfresh (gensym.init hf) n).1) :=
+begin
+  intro h,
+  cases n,
+  { simp [gensym.nfresh, tx3, tx3_helper] },
+  { simp [tx3],
+    rw gensym.nfresh_succ_eq_nfresh_fresh (gensym.init hf),
+    unfold tx3_helper,
+    simp [h, gensym.length_list_nfresh] }
+end
+
+theorem tx3_correct {f : nat → (literal V)} (hf : injective f) (n : nat) :
+  cnf.equisatisfiable (tx3 hf n) (xor_cnf (gensym.nfresh (gensym.init hf) n).1) :=
+begin
+  unfold tx3,
+  induction n using nat.case_strong_induction_on with n ih,
+  { simp [tx3, tx3_helper, gensym.nfresh] },
+  { simp at ih,
+    by_cases h : n.succ ≤ 3,
+    { exact tx3_base_case hf h },
+    { 
+
+      rw gensym.nfresh_succ_eq_nfresh_fresh (gensym.init hf),
+      unfold tx3_helper,
+      simp [h, gensym.length_list_nfresh],
+
+    }
+  }
+  /-
+  by_cases h : n ≤ 3,
+  { exact tx3_base_case hf h },
+  { cases n,
+    { simp at h, contradiction },
+    {
+      simp [tx3],
+      rw gensym.nfresh_succ_eq_nfresh_fresh (gensym.init hf),
+      unfold tx3_helper,
+      simp [h, gensym.length_list_nfresh],
+      split,
+      { sorry, },
+      {
+        rintros ⟨α, ha⟩,
+
+      }
+    }
+    -/
+  }
+end
+/-
+lemma tseitin_base_case {f : V → nat} (hf : bijective f) {l : list (literal V)} : 
+  length l ≤ 3 → cnf.equisatisfiable (tseitin_xor3 hf l (clause.vars l)) (xor_cnf l) :=
+begin
+  intro h,
+  cases l,
+  { simp [tseitin_xor3, xor_cnf] },
+  { unfold tseitin_xor3, simp [h] }
+end
+
+theorem equisatisfiable_tseitin_xor3 {f : V → nat} (hf : bijective f) (l : list (literal V)) :
+  assignment.equisatisfiable (λ α, cnf.eval α (tseitin_xor3 hf l (clause.vars l)))
+                             (λ α, cnf.eval α (xor_cnf l)) :=
+begin
+  cases l,
+  { simp [tseitin_xor3, xor_cnf], 
+    split;
+    { rintros ⟨α, ha⟩,
+      simp at ha,
+      contradiction } },
+  { by_cases h : (length (l_hd :: l_tl) ≤ 3),
+    { split,
+      { rintros ⟨α, ha⟩,
+        unfold tseitin_xor3 at ha,
+        simp [h] at ha,
+        use [α, ha] },
+      { rintros ⟨α, ha⟩,
+        simp at ha,
+        unfold tseitin_xor3,
+        use [α],
+        simp [h, ha] } },
+    { split,
+      { rintros ⟨α, ha⟩,
+        unfold tseitin_xor3 at ha,
+        simp [h] at ha,
+
+      }
+
+    }
+  }
 end
 
 -- We start with the instance of pooling number n = 3
 -- The n provided is the greatest element in l, so that new variables can be created
 -- The well_founded had to be used because of the growing n variable
 -- Unfold didn't work until I provided a nil case - intentional?
+/-
 def tseitin_xor3 : list literal → nat → cnf
 | [] _ := [[]]
 | l n := 
@@ -55,85 +260,141 @@ using_well_founded {
 lemma tseitin_xor3_base_case {ls : list literal} (n : nat) (h : length ls ≤ 3) :
   tseitin_xor3 ls n = xor_cnf ls :=
 begin
-  rcases list_by_cases ls with (rfl | ⟨l, ls, rfl⟩),
+  cases ls,
   { simp [tseitin_xor3, xor_cnf] },
   { unfold tseitin_xor3, simp [h] }
 end
 
--- Big theorem
--- Modify to state that the greatest element of ls is its length
--- TODO max var operates on clauses, but this is a list literal, clean up types later
-theorem tseitin_xor3_correct (α : assignment) : ∀ {ls : list literal}, ∀ {n : nat},
-  (map var ls).nodup → n = max_var ls → cnf.eval α (xor_cnf ls) = cnf.eval α (tseitin_xor3 ls n)
-| []   n := by { simp [xor_cnf, tseitin_xor3] }
-| [l]  n := begin
-  intros _ hmax,
-  have hlen : length [l] = 1, simp [length],
-  rw tseitin_xor3_base_case n (eq.trans_le hlen (nat.one_le_bit1 1))
+α : assignment, ls, ∃ a₂ cnf.eval α (tseitn ls)
+
+∀ α, ∃ a₂ s.t. cnf α (xor_cnf ls) = tt → cnf α₂ (tseitn ls) = tt
+            (cnf α (xor_cnf ls) = cnf α₂ (xor_cnf ls) by equiv on domain?)
+               cnf α (xor_cnf ls) = cnf α₂ (tseitin ls)
+
+∀ α, ∃ a₂ st. cnf α (tseitin ls) = tt → cnf α₂ (xor_cnf ls) = tt
+                cnf α₂ (xor_cnf ls) = ff → cnf α (tseitn ls) = ff
+
+theorem tseitin_xor3_correct : ∀ (α : assignment), ∀ (ls : list literal), ∀ (n : nat),
+  n = max_var ls → ∃ (α₂ : assignment) 
+  (H : α ≡[vars ls]≡ α₂),
+  cnf.eval α₂ (xor_cnf ls) = cnf.eval α₂ (tseitin_xor3 ls n)
+| α [] n hmax := begin
+  use α, simp [xor_cnf, tseitin_xor3]
 end
-| (l₁ :: [l₂]) n := begin
-  intros _ _,
-  have hlen : length (l₁ :: [l₂]) = 2, simp [length],
-  rw tseitin_xor3_base_case n (eq.trans_le hlen (nat.le_succ 2))
+| α [l] n hmax := begin
+  use α, split, { exact eqod.refl α (vars [l]) },
+  { have hlen : length [l] = 1, simp [length],
+    rw tseitin_xor3_base_case n (eq.trans_le hlen (nat.one_le_bit1 1)) }
 end
-| (l₁ :: l₂ :: [l₃]) n := begin
-  intros _ _,
-  have hlen : length (l₁ :: l₂ :: [l₃]) = 3, simp [length],
-  rw tseitin_xor3_base_case n (eq.symm hlen).ge
+| α (l₁ :: [l₂]) n hmax := begin
+  use α, split, { exact eqod.refl α _ },
+  { have hlen : length (l₁ :: [l₂]) = 2, simp [length],
+    rw tseitin_xor3_base_case n (eq.trans_le hlen (nat.le_succ 2)) }
 end
-| (l₁ :: l₂ :: l₃ :: l₄ :: l) n := begin
-  intros hnodup hmax,
-  have : 3 < 4, from nat.lt.base 3,
-  have : 3 < (length l) + 4, from nat.lt_add_left 3 4 (length l) this,
-  have hlen : (length l) + 1 + 1 + 1 + 1 > 3, simp [length, this],
-  have hlen2 : ¬((length l) + 1 + 1 + 1 + 1 ≤ 3), from not_le.mpr this,
-  unfold tseitin_xor3,
-  simp [hlen2],
-  have hnodup_original := hnodup,
-  rw map_cons at hnodup,
-  rw map_cons at hnodup,
-  rw map_cons at hnodup,
-  have t1 := nodup_of_nodup_cons hnodup,
-  have t2 := nodup_of_nodup_cons t1,
-  have t3 := nodup_of_nodup_cons t2,
+| α (l₁ :: l₂ :: [l₃]) n hmax := begin
+  use α, split, { exact eqod.refl α _ },
+  { have hlen : length (l₁ :: l₂ :: [l₃]) = 3, simp [length],
+    rw tseitin_xor3_base_case n (eq.symm hlen).ge }
+end
+| α (l₁ :: l₂ :: l₃ :: l₄ :: l) n hmax := begin
 
-  have : (l₁ :: l₂ :: l₃ :: l₄ :: l) ≠ [], from cons_ne_nil l₁ (l₂ :: l₃ :: l₄ :: l),
-  have ngt : n + 1 > n, from lt_add_one n,
+  have pos_not_mem : Pos (n + 1) ∉ (l₁ :: l₂ :: l₃ :: l₄ :: l),
+    { have hg : n + 1 > n, from lt_add_one n,
+      have : (Pos (n + 1)).var = n + 1, simp [var],
+      rw ← this at hg,
+      rw hmax at hg,
+      have := not_mem_of_gt_max_var hg,
+      rw ← hmax at this,
+      exact this },
+  have neg_not_mem : Neg (n + 1) ∉ (l₁ :: l₂ :: l₃ :: l₄ :: l),
+    { have hg : n + 1 > n, from lt_add_one n,
+      have : (Neg (n + 1)).var = n + 1, simp [var],
+      rw ← this at hg,
+      rw hmax at hg,
+      have := not_mem_of_gt_max_var hg,
+      rw ← hmax at this,
+      exact this },
+  have nsucc_not_mem_map_var : n + 1 ∉ map var (l₁ :: l₂ :: l₃ :: l₄ :: l),
+  { apply not_mem_map_var_of_gt_max_var2,
+    rw hmax, exact lt_add_one _ },
+  have nsucc_not_mem : n + 1 ∉ vars (l₁ :: l₂ :: l₃ :: l₄ :: l),
+    from not_mem_vars_iff_not_mem_map_vars.mp nsucc_not_mem_map_var,
+  
+  -- We want to call the IH on the smaller list - say it's a sublist to get nodup
+  have hsublist : map var (l₄ :: l) <+ map var (l₁ :: l₂ :: l₃ :: l₄ :: l),
+    simp [sublist.cons],
+  have nsucc_not_mem_sublist_map_var : n + 1 ∉ map var (l₄ :: l),
+    from not_mem_of_sublist_of_not_mem nsucc_not_mem_map_var hsublist,
 
-  have s1 : max_var (l₂ :: l₃ :: l₄ :: l) ≤ max_var (l₁ :: l₂ :: l₃ :: l₄ :: l), 
-    from max_var_le_max_var_cons _ _,
-  have s2 : max_var (l₃ :: l₄ :: l) ≤ max_var (l₂ :: l₃ :: l₄ :: l),
-    from max_var_le_max_var_cons _ _,
-  have s3 : max_var (l₄ :: l) ≤ max_var (l₃ :: l₄ :: l),
-    from max_var_le_max_var_cons _ _,
-  have s23 : max_var (l₄ :: l) ≤ max_var (l₂ :: l₃ :: l₄ :: l),
-    from le_trans s3 s2,
-  have s13 : max_var (l₄ :: l) ≤ max_var (l₁ :: l₂ :: l₃ :: l₄ :: l),
-    from le_trans s23 s1,
-  rw ← hmax at s13,
-  have succn_gt : n + 1 > max_var (l₄ :: l), from gt_of_gt_of_ge ngt s13,
-  have : (Neg (n + 1)).var = n + 1, simp [var],
+  have dis : disjoint (map var (l₁ :: l₂ :: l₃ :: l₄ :: l)) [n + 1],
+    { apply disjoint_right.mpr,
+      intros a ha,
+      rw eq_of_mem_singleton ha,
+      exact nsucc_not_mem_map_var },
+  have dis2 : disjoint (map var (l₄ :: l)) [n + 1],
+    { apply disjoint_right.mpr,
+      intros a ha,
+      rw eq_of_mem_singleton ha,
+      exact nsucc_not_mem_sublist_map_var },
+  have hnewmax : n + 1 = max_var ((l₁ :: l₂ :: l₃ :: l₄ :: l) ++ [Pos (n + 1)]),
+    { rw max_var_append,
+      rw ← hmax,
+      simp [max_var_singleton, var] },
+  have hnewmax2 : n + 1 = max_var (l₄ :: l ++ [Pos (n + 1)]),
+  { have hsl : l₄ :: l <+ l₁ :: l₂ :: l₃ :: l₄ :: l, simp [sublist.cons],
+    have hgt : max_var [Pos (n + 1)] > max_var (l₁ :: l₂ :: l₃ :: l₄ :: l),
+      { simp [max_var_singleton, ← hmax, var] },
+    have := max_var_sublist_append hsl hgt,
+    simp [max_var_singleton, var] at this,
+    exact this.symm },
+  have hlen : (l₁ :: l₂ :: l₃ :: l₄ :: l).length > 3,
+    simp [length, nat.lt_add_left 3 4 (length l) (nat.lt.base 3)],
 
-  have smallnodup : (map var (l₁ :: l₂ :: l₃ :: [Neg (n + 1)])).nodup,
-  { sorry },
-  have newnodup : (map var (l₄ :: (l ++ [Pos (n + 1)]))).nodup,
-  { sorry },
-  have newmaxvar : n + 1 = max_var (l₄ :: (l ++ [Pos (n + 1)])),
-  { sorry },
+  cases h123 : (xor_gate.eval α (l₁ :: l₂ :: [l₃])),
+  { have hextend := exists_extended_assignment_of_assignment α nsucc_not_mem ff,
+    rcases hextend with ⟨α₂, hequiv, hff⟩,
+    --unfold tseitin_xor3,
+    --simp [not_le.mpr hlen],
+    rcases tseitin_xor3_correct α₂ ((l₄ :: l) ++ [Pos (n + 1)]) (n + 1) hnewmax2 with ⟨a3, ha3, h3eq⟩,
+    have hnewa : α ≡[vars (l₁ :: l₂ :: l₃ :: l₄ :: l)]≡ (λ v, if v ∈ vars (l₁ :: l₂ :: l₃ :: l₄ :: l) then α v else a3 v),
+      { intros v hv, simp [hv] },
+    use [(λ v, if v ∈ vars (l₁ :: l₂ :: l₃ :: l₄ :: l) then α v else a3 v), hnewa],
+    
+    have : cnf.vars (xor_cnf (l₁ :: l₂ :: l₃ :: l₄ :: l)) ⊆ vars (l₁ :: l₂ :: l₃ :: l₄ :: l),
+    { have : l₁ :: l₂ :: l₃ :: l₄ :: l ≠ [], simp,
+      exact subset.trans (vars_cnf_subset_xor this) (map_var_subset_of_vars (l₁ :: l₂ :: l₃ :: l₄ :: l)) },
 
+    have : α ≡[cnf.vars (xor_cnf (l₁ :: l₂ :: l₃ :: l₄ :: l))]≡ (λ v, if v ∈ vars (l₁ :: l₂ :: l₃ :: l₄ :: l) then α v else a3 v),
+      from eqod_subset_of_eqod this hnewa,
 
-  have ihred := tseitin_xor3_correct newnodup newmaxvar,
-  rw cnf.eval_concat,
-  rw ← ihred,
-  rw xor_cnf_correct α hnodup_original,
-  rw xor_cnf_correct α newnodup,
-  rw xor_cnf_correct α smallnodup,
-  simp [xor_gate.eval_cons, xor_gate.eval_concat],
-  rcases bool_by_cases (eval α (Pos (n + 1))) with htt | hff,
-  {
-    simp [literal.eval] at htt,
-    simp [htt, bxor_ff, literal.eval],
+    rw ← eval_eq_of_equiv_on_domain_vars this,
+    unfold tseitin_xor3,
+    simp [not_le.mpr hlen],
+    rw eval_append,
+
+    --have : cnf.eval (λ v, ite (v ∈ vars (l₁ :: l₂ :: l₃ :: l₄ :: l) (α v) (a3 v))) (xor_cnf (l₁ :: l₂ :: l₃ :: l₄ ))
+    --rw eval_append,
+      
+    --rw xor_cnf_correct α₂ (l₁ :: l₂ :: l₃ :: l₄ :: l),
+   -- rw xor_cnf_correct α₂ [l₁, l₂, l₃, Neg (n + 1)],
+
+    have : cnf.vars (xor_cnf (l₄ :: l ++ [Pos (n + 1)])) ⊆ clause.vars (l₄ :: l ++ [Pos (n + 1)]),
+    { have : (l₄ :: l ++ [Pos (n + 1)]) ≠ [], simp,
+      have h : map var (l₄ :: l ++ [Pos (n + 1)]) ⊆ clause.vars (l₄ :: l ++ [Pos (n + 1)]),
+        from map_var_subset_of_vars (l₄ :: l ++ [Pos (n + 1)]),
+      exact subset.trans (vars_cnf_subset_xor this) h },
+    
+    have h3equivnew : α₂ ≡[cnf.vars (xor_cnf (l₄ :: l ++ [Pos (n + 1)]))]≡ a₃,
+      from eqod_subset_of_eqod this h3equiv,
+
+    have evala3 : cnf.eval α₂ (xor_cnf (l₄ :: l ++ [Pos (n + 1)])) = cnf.eval a₃ (xor_cnf (l₄ :: l ++ [Pos (n + 1)])),
+      from eval_eq_of_equiv_on_domain_vars h3equivnew,
+    }
   }
 end
+-/
+-/
+-/
+-/
 
 end tseitin_xor
