src/xor/xor.lean
@@ -17,16 +17,16 @@ import cnf.cnf
 import cnf.explode
 import basic
 
-/- An n-literal XOR gate is a list of those literals -/
-def xor_gate := list literal
-
-namespace xor_gate
-
 open list
 open literal
 open clause
 open cnf
 open explode
+
+/- An n-literal XOR gate is a list of those literals -/
+def xor_gate := list literal
+
+namespace xor_gate
 
 instance : has_append xor_gate := ⟨list.append⟩
 
@@ -44,16 +44,42 @@ by simp [to_clause]
 def eval (α : assignment) (g : xor_gate) : bool :=
   g.foldr (λ l b, b ⊕ l.eval α) ff
 
-@[simp] lemma eval_nil (α : assignment) : eval α [] = ff := rfl
+def eval2 (α : assignment) (g : xor_gate) : bool :=
+  foldr bxor ff (map (literal.eval α) g)
 
-lemma eval_cons (α : assignment) (l : literal) (g : xor_gate) : eval α (l :: g) = bxor (literal.eval α l) (eval α g) :=
+@[simp] theorem eval_nil (α : assignment) : eval α [] = ff := rfl
+
+theorem eval_cons (α : assignment) (l : literal) (g : xor_gate) : eval α (l :: g) = bxor (literal.eval α l) (eval α g) :=
 by simp [eval, foldr_cons, bool.bxor_comm]
 
-lemma eval_concat (α : assignment) (g₁ g₂ : xor_gate) : eval α (g₁ ++ g₂) = bxor (eval α g₁) (eval α g₂) :=
+@[simp] theorem eval2_nil (α : assignment) : eval2 α [] = ff := rfl
+
+theorem eval2_cons (α : assignment) (l : literal) (g : xor_gate) : eval2 α (l :: g) = bxor (literal.eval α l) (eval2 α g) :=
+by simp [eval2, foldr_cons, bool.bxor_comm]
+
+theorem eval_eq_eval2 (α : assignment) (g : xor_gate) : eval α g = eval2 α g :=
+begin
+  induction g with l ls ih,
+  { simp },
+  { simp only [eval_cons, eval2_cons, ih] }
+end
+
+theorem eval_concat (α : assignment) (g₁ g₂ : xor_gate) : eval α (g₁ ++ g₂) = bxor (eval α g₁) (eval α g₂) :=
 begin
   induction g₁ with l ls ih,
   { simp },
   { simp [eval_cons, ih] }
+end
+
+theorem eval_perm (α : assignment) {g₁ g₂ : xor_gate} :
+  g₁ ~ g₂ → eval α g₁ = eval α g₂ :=
+begin
+  intro h,
+  have : (map (literal.eval α) g₁) ~ (map (literal.eval α) g₂),
+  { exact perm.map (literal.eval α) h },
+  rw eval_eq_eval2,
+  rw eval_eq_eval2,
+  exact perm.foldr_eq (bool.bxor_left_comm) this ff
 end
 
 theorem eval_cons_conjunctive (α : assignment) (l : literal) (g : xor_gate) : 
@@ -82,7 +108,7 @@ theorem xor_odd_eval_tt (α : assignment) (g : xor_gate) : g.eval α = nat.bodd 
 begin
   induction g with l ls ih,
   { simp },
-  { rcases bool_by_cases (l.eval α) with h | h;
+  { cases h : (l.eval α);
     { simp [eval_cons, h, ih] } }
 end
 
@@ -93,7 +119,7 @@ theorem xor_odd_eval_tt2 (α : assignment) (g : xor_gate) : g.eval α = nat.bodd
 begin
   induction g with l ls ih,
   { simp [to_clause] },
-  { rcases bool_by_cases (l.eval α);
+  { cases h : (l.eval α);
     { rw ← gate_eq_clause ls at ih,
       simp [to_clause, eval_cons, count_tt_cons, bool.to_nat, h, ih] } }
 end
@@ -114,8 +140,10 @@ theorem mem_explode_of_mem_nat_to_xor :
   simp [nat_to_xor_cnf, mem_map, mem_append],
   intros c hc,
   have : (Pos n).var = n ∧ (Neg n).var = n, simp [var], -- Make into literal lemma?
-  rcases bool_by_cases (c.count_neg.bodd) with h | h;
-  { simp [h, mem_explode_cons_of_lit c hc, this] }
+  cases h : (c.count_neg.bodd);
+  { simp [h, this],
+    apply mem_explode_cons_of_mem_explode_of_lit,
+    exact hc }
 end
 
 theorem length_nat_to_xor_cnf : ∀ {ns : list nat}, ns ≠ [] → length (nat_to_xor_cnf ns) = 2^(length ns - 1)
@@ -134,7 +162,7 @@ theorem map_var_eq_of_mem_nat_to_xor : ∀ {ns : list nat}, ∀ {c : clause}, c 
 | (n :: ns) := begin
   simp [nat_to_xor_cnf],
   intros c hc,
-  rcases bool_by_cases c.count_neg.bodd;
+  cases h : c.count_neg.bodd;
   { simp [h, var, map_var_eq_of_mem_explode hc] }
 end
 
@@ -158,7 +186,7 @@ theorem even_negation_of_mem_nat_to_xor_of_map_var_eq : ∀ {ns : list nat}, ∀
   simp [nat_to_xor_cnf] at hxor,
   rcases hxor with ⟨a, ha, hacons⟩,
   rcases exists_cons_of_map_cons hc with ⟨l, ls, rfl, hl, hls⟩,
-  rcases bool_by_cases a.count_neg.bodd with h | h;
+  cases h : a.count_neg.bodd;
   { simp [h] at hacons,
     simp [← hacons, count_neg_cons, is_neg, bool.to_nat, h] },
 end
@@ -191,29 +219,28 @@ theorem odd_negation_iff_not_mem_nat_to_xor {ns : list nat} {c : clause} (hc : c
   not_mem_nat_to_xor_cnf_of_odd_negation_of_map_var_eq hc⟩
 
 -- We prove that the naive encoding is equivalent to an XOR gate of all positive literals
-theorem nat_to_xor_cnf_correct (α : assignment) : ∀ {ns : list nat}, 
-  ns.nodup → cnf.eval α (nat_to_xor_cnf ns) = eval α (ns.map Pos)
+theorem nat_to_xor_cnf_correct (α : assignment) : ∀ (ns : list nat), 
+  cnf.eval α (nat_to_xor_cnf ns) = eval α (ns.map Pos)
 | []        := by simp [nat_to_xor_cnf]
 | (n :: ns) := begin
-  intro hnodup,
   have red := xor_odd_eval_tt2 α (map Pos (n :: ns)),
-  rcases bool_by_cases (eval α (map Pos (n :: ns))) with h | h;
-  rw [h, ← gate_eq_clause (map Pos (n :: ns))] at red; rw h,
-  -- tt case: Parities of α and clause tt evals means all clauses are true
-  { apply eval_tt_iff_clauses_tt.mpr,
-    intros c hc,
-    have mve := map_var_eq_of_mem_nat_to_xor hc,
-    have neq := neq_of_ff_of_tt (eq.symm red) ((even_negation_iff_mem_nat_to_xor mve).mp hc),
-    exact eval_tt_of_opposite_parity (cons_ne_nil n ns) hnodup mve neq },
+  cases h : (eval α (map Pos (n :: ns)));
+  rw [h, ← gate_eq_clause (map Pos (n :: ns))] at red,
   -- ff case: We generate a false clause and show it is in the encoded formula
-  { apply eval_ff_iff_exists_clause_ff.mpr,
+  { apply eval_ff_iff_exists_clause_eval_ff.mpr,
     use (falsify α (n :: ns)),
     split,
     { apply (even_negation_iff_mem_nat_to_xor (map_var_falsify_eq_list α (n :: ns))).mpr,
       have oddeq := congr_arg nat.bodd (count_tt_pos_eq_count_neg_falsify α (n :: ns)),
       rw ← red at oddeq,
       exact oddeq.symm },
-    { exact eval_ff_of_falsify α (n :: ns) } }
+    { exact falsify_eval_ff α (n :: ns) } },
+  -- tt case: Parities of α and clause tt evals means all clauses are true
+  { apply eval_tt_iff_forall_clause_eval_tt.mpr,
+    intros c hc,
+    have mve := map_var_eq_of_mem_nat_to_xor hc,
+    have neq := neq_of_ff_of_tt (eq.symm red) ((even_negation_iff_mem_nat_to_xor mve).mp hc),
+    exact eval_tt_of_opposite_parity (cons_ne_nil n ns) mve neq }
 end
 
 /-! # More complex encoding -/
@@ -227,18 +254,22 @@ def xor_cnf : list literal → cnf
 | []        := [[]]
 | (l :: ls) := (explode (map var ls)).map (λ c, cond (nat.bodd (c.count_flips (ls)) = ff) (l :: c) (l.flip :: c))
 
+@[simp] theorem xor_cnf_singleton (l : literal) : xor_cnf [l] = [[l]] :=
+by simp [xor_cnf]
+
 theorem mem_explode_of_mem_xor_cnf :
   ∀ {ls : list literal} {c : clause}, c ∈ xor_cnf ls → c ∈ explode (map var ls)
 | []        := by simp [xor_cnf]
 | (l :: ls) := begin
   simp [xor_cnf, explode],
   intros c hc,
-  rcases exists_nat_of_lit l with ⟨n, (rfl | rfl)⟩;
-  rcases bool_by_cases (nat.bodd (c.count_flips ls)) with h | h,
-  { right, use c, simp [h, hc, var, literal.flip] },
-  { left, use c, simp [h, hc, var, literal.flip] },
-  { left, use c, simp [h, hc, var, literal.flip] },
-  { right, use c, simp [h, hc, var, literal.flip] }
+  cases l,
+  { cases h : (nat.bodd (c.count_flips ls)),
+    { use c, simp [h, hc, var, literal.flip] },
+    { right, use c, simp [h, hc, var, literal.flip] } },
+  { cases h : (nat.bodd (c.count_flips ls)), 
+    { right, use c, simp [h, hc, var, literal.flip] },
+    { use c, simp [h, hc, var, literal.flip] } }
 end
 
 theorem length_xor_cnf : ∀ {ls : list literal}, ls ≠ [] → length (xor_cnf ls) = 2^(length ls - 1)
@@ -258,10 +289,11 @@ begin
   { simp [xor_cnf] },
   { simp [xor_cnf],
     intros c hc,
-    rcases bool_by_cases (nat.bodd (c.count_flips ls)) with h | h;
-    { simp [h, map_var_eq_of_mem_explode hc, var_flip_eq_var l] } }
+    cases h : (nat.bodd (c.count_flips ls));
+    { simp [h, map_var_eq_of_mem_explode hc, flip_var_eq l] } }
 end
 
+-- TODO choose to add back in lemmas on flips for literal
 theorem mem_xor_cnf_of_even_flips_of_map_var_eq : ∀ {ls : list literal}, ∀ {c : clause},
   map var c = map var ls → (nat.bodd (c.count_flips ls) = ff) → c ∈ xor_cnf ls
 | []        := by simp [xor_cnf]
@@ -270,15 +302,22 @@ theorem mem_xor_cnf_of_even_flips_of_map_var_eq : ∀ {ls : list literal}, ∀ {
   intros c hc hcount,
   rcases exists_cons_of_map_cons hc with ⟨d, ds, rfl, hd, hds⟩,
   use ds,
-  rcases bool_by_cases (nat.bodd (count_flips ds ls)) with htt | hff,
+  cases htf : (nat.bodd (count_flips ds ls)),
   { by_cases l.flip = d,
-    { simp [htt, mem_explode_of_map_var_eq hds, hd, h] },
-    { simp [count_flips, ne.symm (ne_flip_of_flip_ne h)] at hcount,
-      exact absurd_bool htt hcount } },
+    { have : d.flip = l, from congr_arg literal.flip h ▸ flip_flip l,
+      simp [count_flips, this] at hcount,
+      exact absurd_bool hcount htf },
+    { simp [htf, mem_explode_of_map_var_eq hds, hd], --eq_of_flip_ne_of_var_eq hd.symm h]
+      rcases eq_or_flip_eq_of_var_eq hd with rfl | h₂,
+      { refl },
+      { have : d = l.flip, from congr_arg literal.flip h₂ ▸ (flip_flip d).symm, 
+        exact absurd this (ne.symm h) } } },
   { by_cases l.flip = d,
-    { simp [count_flips, eq_flip_of_flip_eq h] at hcount,
-      exact absurd_bool hcount hff },
-    { simp [hff, mem_explode_of_map_var_eq hds, hd, eq_of_flip_ne_of_var_eq hd.symm h] } }
+    { simp [htf, mem_explode_of_map_var_eq hds, hd, h], },
+    { have := function.injective.ne flip_injective h,
+      rw flip_flip at this,
+      simp [count_flips, ne.symm this] at hcount,
+      exact absurd_bool htf hcount } }
 end
 
 theorem even_flips_of_mem_xor_cnf_of_map_var_eq : ∀ {ls : list literal}, ∀ {c : clause},
@@ -289,9 +328,9 @@ theorem even_flips_of_mem_xor_cnf_of_map_var_eq : ∀ {ls : list literal}, ∀ {
   simp [xor_cnf] at hxor,
   rcases hxor with ⟨a, ha, hacons⟩,
   rcases exists_cons_of_map_cons hc with ⟨c, cs, rfl, hc2, hcs⟩,
-  rcases bool_by_cases (nat.bodd (count_flips a ls)) with h | h;
+  cases h : (nat.bodd (count_flips a ls));
   { simp [h] at hacons,
-    simp [← hacons, count_flips, is_neg, bool.to_nat, h, eq_flip_flip _, ne_flip_self] }
+    simp [← hacons, count_flips, is_neg, bool.to_nat, h, flip_flip _, flip_ne] }
 end
 
 theorem even_flips_iff_mem_xor_cnf {ls : list literal} {c : clause} (hc : c.map var = map var ls) :
@@ -321,29 +360,131 @@ theorem odd_flips_iff_not_mem_xor_cnf {ls : list literal} {c : clause} (hc : map
 
 -- A restatement of the above theorem in a more general way
 -- Alternatively, the assignment can be manipulated by flipping the correct literals
-theorem xor_cnf_correct (α : assignment) : ∀ {ls : list literal},
-  (map var ls).nodup → cnf.eval α (xor_cnf ls) = eval α ls
+theorem xor_cnf_correct (α : assignment) : ∀ (ls : list literal),
+  cnf.eval α (xor_cnf ls) = eval α ls
 | []        := by simp [xor_cnf]
 | (l :: ls) := begin
-  intro hnodup,
   have red := xor_odd_eval_tt2 α (l :: ls),
-  rcases bool_by_cases (eval α (l :: ls)) with h | h;
-  rw [h, ← gate_eq_clause (l :: ls)] at red; rw h,
-  { apply eval_tt_iff_clauses_tt.mpr,
-    intros c hc,
-    have mve := map_var_eq_of_mem_xor_cnf hc,
-    have neqodd := neq_of_ff_of_tt (eq.symm red) ((even_flips_iff_mem_xor_cnf mve).mpr hc),
-    have neq := ne_of_apply_ne nat.bodd neqodd,
-    rw count_flips_comm at neq,
-    exact eval_tt_of_neq_flips (cons_ne_nil l ls) hnodup c mve.symm neq },
-  { apply eval_ff_iff_exists_clause_ff.mpr,
+  cases h : (eval α (l :: ls));
+  rw [h, ← gate_eq_clause (l :: ls)] at red,
+  { apply eval_ff_iff_exists_clause_eval_ff.mpr,
     use (falsify α (map var (l :: ls))),
     split,
     { rw ← count_flips_falsify_eq_count_tt α (l :: ls) at red,
       rw count_flips_comm at red,
       apply (even_flips_iff_mem_xor_cnf (map_var_falsify_eq_list α (map var (l :: ls)))).mp,
       exact red.symm },
-    { exact eval_ff_of_falsify α (map var (l :: ls)) } }
+    { exact falsify_eval_ff α (map var (l :: ls)) } },
+  { apply eval_tt_iff_forall_clause_eval_tt.mpr,
+    intros c hc,
+    have mve := map_var_eq_of_mem_xor_cnf hc,
+    have neqodd := neq_of_ff_of_tt (eq.symm red) ((even_flips_iff_mem_xor_cnf mve).mpr hc),
+    have neq := ne_of_apply_ne nat.bodd neqodd,
+    rw count_flips_comm at neq,
+    exact eval_tt_of_neq_flips (cons_ne_nil l ls) c mve.symm neq }
+end
+
+theorem vars_cnf_subset_xor {ls : list literal} :
+  ls ≠ [] → cnf.vars (xor_cnf ls) ⊆ (map var ls) :=
+begin
+  intro h,
+  cases ls,
+  { contradiction },
+  { intros n hn,
+    rcases cnf.exists_mem_clause_of_mem_vars hn with ⟨c, hcnf, hc⟩,
+    simp [← map_var_eq_of_mem_xor_cnf hcnf, mem_vars_iff_mem_map_vars, hc] }
+end
+
+end xor_gate
+
+/-! # Equivalence on domain for this encoding -/
+
+namespace assignment
+
+theorem equiv_on_domain_for_xor {α₁ α₂ : assignment} : ∀ {ls : list literal},
+  (α₁ ≡[map var ls]≡ α₂) → xor_gate.eval α₁ ls = xor_gate.eval α₂ ls :=
+begin
+  intros ls heq,
+  cases ls,
+  { simp },
+  { have := eqod_subset_of_eqod (xor_gate.vars_cnf_subset_xor (cons_ne_nil ls_hd ls_tl)) heq,
+    simp [← xor_gate.xor_cnf_correct α₁, 
+      ← xor_gate.xor_cnf_correct α₂, eval_eq_of_equiv_on_domain_vars this] }
+end
+
+end assignment
+
+namespace xor_gate
+
+theorem exists_assignment_eval_tt_of_nodup {l : list literal} :
+  l ≠ [] → nodup (map var l) → ∃ (α : assignment), eval α l = tt :=
+begin
+  induction l with l ls ih,
+  { simp },
+  { intros _ hnodup,
+    cases ls,
+    { cases l,
+      { use assignment.all_tt, simp [eval, literal.eval, assignment.all_tt_eval_tt] },
+      { use assignment.all_ff, simp [eval, literal.eval, assignment.all_ff_eval_ff] } },
+    { rw map_cons at hnodup,
+      rcases ih (cons_ne_nil _ _) (nodup_of_nodup_cons hnodup) with ⟨α, ha⟩,
+      cases l,
+      { have : (λ x, if x = l then ff else α x) ≡[map var (ls_hd :: ls_tl)]≡ α,
+        { intros x hx,
+          unfold var at hnodup,
+          have : l ∉ (map var (ls_hd :: ls_tl)), from not_mem_of_nodup_cons hnodup,
+          by_cases h : x = l,
+          { rw ← h at this, exact absurd hx this },
+          { simp [h] } },
+        use (λ x, if x = l then ff else α x),
+        rw xor_gate.eval_cons,
+        simp [literal.eval, assignment.equiv_on_domain_for_xor this, ha] },
+      { have : (λ x, if x = l then tt else α x) ≡[map var (ls_hd :: ls_tl)]≡ α,
+        { intros x hx,
+          unfold var at hnodup,
+          have : l ∉ (map var (ls_hd :: ls_tl)), from not_mem_of_nodup_cons hnodup,
+          by_cases h : x = l,
+          { rw ← h at this, exact absurd hx this },
+          { simp [h] } },
+        use (λ x, if x = l then tt else α x),
+        rw xor_gate.eval_cons,
+        simp [literal.eval, assignment.equiv_on_domain_for_xor this, ha] } } }
+end
+
+theorem exists_assignment_eval_ff_of_nodup {l : list literal} :
+  l ≠ [] → nodup (map var l) → ∃ (α : assignment), eval α l = ff :=
+begin
+  intros hnil hnodup,
+  rcases exists_cons_of_ne_nil hnil with ⟨l, ls, rfl⟩,
+  rw map_cons at hnodup,
+  cases ls,
+  { cases l, 
+    { use assignment.all_ff,
+      simp [eval, assignment.all_ff_eval_ff, literal.eval] },
+    { use assignment.all_tt,
+      simp [eval, assignment.all_tt_eval_tt, literal.eval] } },
+  { rcases exists_assignment_eval_tt_of_nodup (cons_ne_nil ls_hd ls_tl) (nodup_of_nodup_cons hnodup) with ⟨α, ha⟩,
+    cases l,
+    { use (λ x, if x = l then tt else α x),
+      have : (λ x, if x = l then tt else α x) ≡[map var (ls_hd :: ls_tl)]≡ α,
+      { intros x hx,
+          unfold var at hnodup,
+          have : l ∉ (map var (ls_hd :: ls_tl)), from not_mem_of_nodup_cons hnodup,
+          by_cases h : x = l,
+          { rw ← h at this, exact absurd hx this },
+          { simp [h] } },
+      rw eval_cons,
+      simp [literal.eval, assignment.equiv_on_domain_for_xor this, ha] },
+    { use (λ x, if x = l then ff else α x),
+      have : (λ x, if x = l then ff else α x) ≡[map var (ls_hd :: ls_tl)]≡ α,
+      { intros x hx,
+          unfold var at hnodup,
+          have : l ∉ (map var (ls_hd :: ls_tl)), from not_mem_of_nodup_cons hnodup,
+          by_cases h : x = l,
+          { rw ← h at this, exact absurd hx this },
+          { simp [h] } },
+      rw eval_cons,
+      simp [literal.eval, assignment.equiv_on_domain_for_xor this, ha] } }
 end
 
 end xor_gate
