src/cnf/assignment_general.lean
@@ -1,0 +1,153 @@
+/-
+Defines the properties of assignments on general variables.
+
+Authors: Cayden Codel, Jeremy Avigad, Marijn Heule
+Carnegie Mellon University
+-/
+
+import data.list.basic
+import cnf.literal_general
+
+universe u
+
+variables {V : Type u} [decidable_eq V] [inhabited V]
+
+namespace assignment
+
+open literal
+open list
+
+-- This is giving me some trouble when moving to the general case
+--instance : inhabited assignment := ⟨(λ _, tt)⟩
+
+/-! # Equisatisfiability -/
+
+/- Formulas are functions from assignments to booleans
+   Two formulas are equisatisfiable if the satisfiability of one
+   implies the satisfiability of the other.
+-/
+def equisatisfiable (f₁ f₂ : assignment V → bool) : Prop := 
+  (∃ (α₁ : assignment V), f₁ α₁ = tt) ↔ (∃ (α₂ : assignment V), f₂ α₂ = tt)
+
+/-! # Equivalence on domain -/
+
+def eqod (α₁ α₂ : assignment V) (l : list V) : Prop := ∀ v ∈ l, α₁ v = α₂ v
+
+-- Better notation for this?
+notation α₁ ` ≡[`:50 l `]≡ `:50 α₂ := eqod α₁ α₂ l
+
+@[refl] theorem eqod.refl (α : assignment V) (l : list V) : α ≡[l]≡ α :=
+by simp [eqod]
+
+@[symm] theorem eqod.symm {α₁ α₂ : assignment V} {l : list V} (p : α₁ ≡[l]≡ α₂) :
+  α₂ ≡[l]≡ α₁ :=
+assume v hv, (p v hv).symm
+
+theorem eqod_comm {α₁ α₂ : assignment V} {l : list V} :
+  (α₁ ≡[l]≡ α₂) ↔ (α₂ ≡[l]≡ α₁) :=
+⟨eqod.symm, eqod.symm⟩
+
+@[trans] theorem eqod.trans {α₁ α₂ α₃ : assignment V} {l : list V} :
+  (α₁ ≡[l]≡ α₂) → (α₂ ≡[l]≡ α₃) → (α₁ ≡[l]≡ α₃) :=
+assume h₁ h₂ v hv, eq.trans (h₁ v hv) (h₂ v hv)
+
+/-! # General properties -/
+
+@[simp] theorem eqod_nil (α₁ α₂ : assignment V) : α₁ ≡[nil]≡ α₂ :=
+by simp [eqod]
+
+-- If domains become sets instead of lists, then perms become moot
+theorem eqod_perm {α₁ α₂ : assignment V} {l₁ l₂ : list V} :
+  l₁ ~ l₂ → (α₁ ≡[l₁]≡ α₂) → α₁ ≡[l₂]≡ α₂ :=
+assume h₁ h₂ v hv, h₂ v ((perm.mem_iff h₁).mpr hv)
+
+theorem eqod_of_eqod_cons {α₁ α₂ : assignment V} {v : V} {l : list V} :
+  (α₁ ≡[v :: l]≡ α₂) → α₁ ≡[l]≡ α₂ :=
+by simp [eqod]
+
+-- From the set point of view, we might want non-membership of new value v
+theorem eqod_cons_of_eq_of_not_mem_of_eqod {α₁ α₂ : assignment V} {v : V} {l : list V} :
+  (α₁ ≡[l]≡ α₂) → α₁ v = α₂ v → α₁ ≡[v :: l]≡ α₂ :=
+begin
+  intros h₁ heq m hm,
+  rcases eq_or_mem_of_mem_cons hm with rfl | hml,
+  { exact heq },
+  { exact h₁ m hml }
+end
+
+theorem eqod_subset_of_eqod {α₁ α₂ : assignment V} {l₁ l₂ : list V} :
+  l₁ ⊆ l₂ → (α₁ ≡[l₂]≡ α₂) → α₁ ≡[l₁]≡ α₂ :=
+assume h₁ h₂ v hv, h₂ v (h₁ hv)
+
+-- The types of mem_union don't check?
+--theorem eqod_union_of_eqod [decidable_eq V] [has_union (list V)] [has_mem V (list V)] {α₁ α₂ : assignment V} {l₁ l₂ : list V} :
+--  (α₁ ≡[l₁]≡ α₂) → (α₁ ≡[l₂]≡ α₂) → α₁ ≡[l₁ ∪ l₂]≡ α₂ :=
+--assume h₁ h₂ v hv, by { cases (mem_union.mp hn), exact h₁ n h, exact h₂ n h }
+
+-- Same thing here, with mem_inter
+--theorem eqod_inter_of_eqod [has_inter (list V)] {α₁ α₂ : assignment V} {l₁ l₂ : list V} :
+--  (α₁ ≡[l₁]≡ α₂) → (α₁ ≡[l₂]≡ α₂) → α₁ ≡[l₁ ∩ l₂]≡ α₂ :=
+--assume h₁ _ v hv, h₁ v (mem_inter.mp hv).1
+
+theorem eqod_append_left {α₁ α₂ : assignment V} {l₁ l₂ : list V} :
+  (α₁ ≡[l₁ ++ l₂]≡ α₂) → α₁ ≡[l₁]≡ α₂ :=
+assume h, eqod_subset_of_eqod (sublist.subset (sublist_append_left l₁ l₂)) h
+
+theorem eqod_append_right {α₁ α₂ : assignment V} {l₁ l₂ : list V} :
+  (α₁ ≡[l₁ ++ l₂]≡ α₂) → α₁ ≡[l₂]≡ α₂ :=
+assume h, eqod_subset_of_eqod (sublist.subset (sublist_append_right l₁ l₂)) h
+
+/-! # Evaluation and extension -/
+
+theorem eval_eq_of_mem_of_eqod {α₁ α₂ : assignment V} {l : list V} {lit : literal V} :
+  (α₁ ≡[l]≡ α₂) → lit.var ∈ l → literal.eval α₁ lit = literal.eval α₂ lit :=
+by { cases lit; simp only [literal.eval, var]; intros h hl; simp only [h lit hl] }
+
+-- Sometimes the domain of equivalence needs to be extended according to a particular assignment
+theorem exists_extended_assignment_of_assignment [decidable_eq V] (α₁ : assignment V) {l : list V} {v : V} :
+  v ∉ l → ∀ (b : bool), ∃ (α₂ : assignment V), (α₁ ≡[l]≡ α₂) ∧ α₂ v = b :=
+begin
+  intros hv b,
+  use (λ (x : V), if x = v then b else α₁ x),
+  simp [eqod],
+  intros x hx,
+  simp [ne_of_mem_of_not_mem hx hv]
+end
+
+-- The domain can be extended by whole lists instead
+theorem exists_list_extended_assignment_of_assignment [decidable_eq V] (α₁ : assignment V) {l e : list V} :
+  disjoint l e → ∀ (f : V → bool), ∃ (α₂ : assignment V), (α₁ ≡[l]≡ α₂) ∧ (∀ n ∈ e, α₂ n = f n) :=
+begin
+  intros hle f,
+  use (λ x, if x ∈ e then f x else α₁ x),
+  simp [eqod],
+  split,
+  { intros v hv, simp [hle hv] },
+  { intros n ha hb, contradiction }
+end
+
+/-! # Miscellaneous -/
+
+-- Constant function assignments
+def all_tt : assignment V := (λ _, tt)
+def all_ff : assignment V := (λ _, ff)
+
+theorem all_tt_eval_tt : ∀ (n : V), all_tt n = tt := by simp [all_tt]
+theorem all_ff_eval_ff : ∀ (n : V), all_ff n = ff := by simp [all_ff]
+
+-- There may be times where setting or flipping variables is important
+def set_var [decidable_eq V] (α : assignment V) (v : V) (b : bool) : assignment V :=
+  λ x, if x = v then b else α x
+
+def flip_var [decidable_eq V] (α : assignment V) (v : V) : assignment V :=
+  λ x, if x = v then bnot (α v) else α x
+
+theorem eval_eq_of_set_var [decidable_eq V] {α : assignment V} {v : V} {b : bool} : 
+  (set_var α v b) v = b :=
+by simp [set_var]
+
+theorem eval_ne_of_flip_var [decidable_eq V] {α : assignment V} {v : V} :
+  α v = bnot ((flip_var α v) v) :=
+by simp [flip_var]
+
+end assignment
