src/cnf/gensym.lean
@@ -1,0 +1,502 @@
+/-
+Following the tradition of other programming languages,
+gensym.lean contains the definition and proofs for a
+variable generator for CNF encodings.
+
+Authors: Cayden Codel, Jeremy Avigad, Marijn Heule
+Carnegie Mellon University
+-/
+
+import cnf.cnf_general
+import data.list.basic
+import logic.function.basic
+import data.nat.basic
+
+open function
+open prod
+open list
+
+universe u
+
+variable {α : Type u}
+
+/- A gensym is defined by
+
+    - offset: How far along the gensym has assigned variables
+    - delta: How much the offset is changed by each assignment
+    - f: Convert from nats to desired variable types
+    - h: Proof of injectivity, so variable assignments don't conflict
+
+  The update rule is simple: offset + delta.
+-/
+structure gensym (α : Type u) :=
+(offset : nat)
+(delta : nat)
+(f : nat → α)
+(delta_pos : delta > 0) -- Make into subtypes of delta and f?
+(f_inj : injective f)
+
+namespace gensym
+
+/-! # Instance properties -/
+
+/- Two gensyms are equal if their component parts agree -/
+--@[derive equivalence] <-- This doesn't work - how come?
+-- Theorem g₁ = g₂ iff ... below
+-- congr_xxx 
+protected def eq (g₁ g₂ : gensym α) := g₁.1 = g₂.1 ∧ g₁.2 = g₂.2 ∧ g₁.3 = g₂.3
+
+/-
+cases g
+g = {offset := g.offset, delta := g.delta, f := g.f }
+-/
+
+@[refl] theorem eq.refl (g : gensym α) : g = g := rfl
+
+@[symm] theorem eq.symm {g₁ g₂ : gensym α} (p : g₁ = g₂) : g₂ = g₁ :=
+by simp [p]
+
+theorem eq_comm {g₁ g₂ : gensym α} : g₁ = g₂ ↔ g₂ = g₁ :=
+⟨eq.symm, eq.symm⟩
+
+@[trans] theorem eq.trans {g₁ g₂ g₃ : gensym α} : g₁ = g₂ → g₂ = g₃ → g₁ = g₃ :=
+eq.trans -- This doesn't seem sketchy at all...
+
+/- For some reason, the above doesn't work.... -/
+def equiv (g₁ g₂ : gensym α) := g₁.1 = g₂.1 ∧ g₁.3 = g₂.3
+
+notation g₁ ` ≃ ` g₂ := equiv g₁ g₂
+
+@[refl] theorem equiv.refl (g : gensym α) : g ≃ g :=
+by simp [equiv]
+
+@[symm] theorem equiv.symm {g₁ g₂ : gensym α} (p : g₁ ≃ g₂) : g₂ ≃ g₁ :=
+begin
+  unfold equiv at p,
+  simp [equiv, p]
+end
+
+theorem equiv_comm {g₁ g₂ : gensym α} : g₁ ≃ g₂ ↔ g₂ ≃ g₁ :=
+⟨equiv.symm, equiv.symm⟩
+
+@[trans] theorem equiv.trans {g₁ g₂ g₃ : gensym α} : g₁ ≃ g₂ → g₂ ≃ g₃ → g₁ ≃ g₃ :=
+begin
+  simp [equiv],
+  intros ho₁ hf₁ ho₂ hf₂,
+  simp [ho₁, hf₁, ho₂, hf₂]
+end
+
+theorem equiv_of_eq {g₁ g₂ : gensym α} : g₁ = g₂ → g₁ ≃ g₂ :=
+assume h, by simp [h]
+
+/-! # Gensym creation -/
+
+/- Initial gensym that starts at 0 -/
+def init {f : nat → α} (f_inj : injective f) : gensym α :=
+{ offset := 0, delta := 1, f := f, delta_pos := nat.one_pos, f_inj := f_inj }
+
+/- Given explicit functions between the two types that are inverses of each other,
+    we create a gensym object that starts at one more than the maximum of the given list. -/
+def seed {f : nat → α} (f_inj : injective f) {g : α → nat} (g_inj : injective g)
+  (rinv : right_inverse f g)
+ : list α → gensym α
+| [] := init f_inj
+| l  := { offset := 1 + max_nat (map g l), 
+          delta := 1, f := f, delta_pos := nat.one_pos, f_inj := f_inj }
+
+@[simp] theorem seed_nil_eq_init {f : nat → α} (f_inj : injective f) 
+  {g : α → nat} (g_inj : injective g) (rinv : right_inverse f g) :
+  seed f_inj g_inj rinv [] ≃ init f_inj :=
+by simp [seed, init]
+
+/-! ### Fresh variable generation -/
+
+/-! # fresh -/
+
+-- Generates a new variable and returns an updated gensym
+def fresh (g : gensym α) : (α × gensym α) :=
+⟨g.f (g.offset), ⟨g.offset + g.delta, g.delta, g.f, g.delta_pos, g.f_inj⟩⟩
+
+@[simp] theorem fresh_offset (g : gensym α) :
+  (fresh g).2.offset = g.offset + g.delta :=
+by simp [fresh]
+
+@[simp] theorem fresh_delta (g : gensym α) : 
+  (fresh g).2.delta = g.delta :=
+by simp [fresh]
+
+@[simp] theorem fresh_f (g : gensym α) : (fresh g).2.f = g.f :=
+by simp [fresh]
+
+theorem fresh_delta_pos (g : gensym α) :
+  (fresh g).2.delta > 0 :=
+(fresh g).2.delta_pos
+
+theorem fresh_f_injective (g : gensym α) :
+  injective (fresh g).2.f :=
+(fresh g).2.f_inj
+
+/-! # nfresh -/
+
+/- Generates a list of n new variables and returns the gensym at the end -/
+def nfresh : gensym α → nat → (list α × gensym α)
+| g 0       := ⟨[], g⟩
+| g (n + 1) := let ⟨a, g₂⟩ := fresh g in
+               prod.map (λ l, a :: l) id (nfresh g₂ n)
+
+@[simp] theorem nfresh_zero (g : gensym α) : nfresh g 0 = ⟨[], g⟩ := rfl
+
+@[simp] theorem nfresh_one (g : gensym α) : (nfresh g 1).2 = (fresh g).2 :=
+by simp [nfresh, fresh]
+
+@[simp] theorem nfresh_offset (g : gensym α) (n : nat) :
+  (nfresh g n).2.offset = (g.delta * n) + g.offset :=
+begin
+  induction n with n ih generalizing g,
+  { simp [nfresh] },
+  { simp [nfresh, fresh, ih],
+    rw [add_comm g.offset g.delta, ← add_assoc, nat.succ_eq_add_one],
+    simp [mul_add] }
+end
+
+@[simp] theorem nfresh_delta (g : gensym α) (n : nat) : 
+  (nfresh g n).2.delta = g.delta :=
+begin
+  induction n with n ih generalizing g,
+  { simp [nfresh] },
+  { simp [nfresh, fresh, ih] }
+end
+
+@[simp] theorem nfresh_f (g : gensym α) (n : nat) : (nfresh g n).2.f = g.f :=
+begin
+  induction n with n ih generalizing g,
+  { simp [nfresh] },
+  { simp [nfresh, fresh, ih] }
+end
+
+theorem nfresh_f_injective (g : gensym α) (n : nat) : injective (nfresh g n).2.f :=
+(nfresh g n).2.f_inj
+
+theorem nfresh_delta_pos (g : gensym α) (n : nat) : (nfresh g n).2.delta > 0 :=
+(nfresh g n).2.delta_pos
+
+theorem nfresh_one_eq_fresh (g : gensym α) : 
+  prod.map (λ a, [a]) id (fresh g) = nfresh g 1 :=
+by simp [fresh, nfresh]
+
+theorem nfresh_succ_eq_nfresh_fresh (g : gensym α) (n : nat) :
+  nfresh g (n + 1) = ⟨(fresh g).1 :: (nfresh (fresh g).2 n).1, (fresh (nfresh g n).2).2⟩ :=
+begin
+  induction n with n ih generalizing g,
+  { simp [nfresh, fresh] },
+  { simp [nfresh, fresh, ih, add_assoc] }
+end
+
+theorem nfresh_succ_gensym_eq_fresh_nfresh_gensym (g : gensym α) (n : nat) :
+  (nfresh g (n + 1)).2 = (fresh (nfresh g n).2).2 :=
+by simp [nfresh_succ_eq_nfresh_fresh]
+
+theorem nfresh_succ_gensym_eq_nfresh_fresh_gensym (g : gensym α) (n : nat) :
+  (nfresh g (n + 1)).2 = (nfresh (fresh g).2 n).2 :=
+by simp [nfresh_succ_eq_nfresh_fresh, nfresh, fresh]
+
+/-
+theorem nfresh_succ_eq_nfresh_append_fresh (g : gensym α) (n : nat) :
+  nfresh g (n + 1) = ⟨(nfresh g n).1 ++ [(fresh (nfresh g n).2).1], (fresh (nfresh g n).2).2⟩ :=
+begin
+  induction n with n ih generalizing g,
+  { simp [nfresh, fresh] },
+  {
+    rw nfresh_succ_eq_nfresh_fresh g (n + 1),
+    rw ih g.fresh.snd,
+    simp,
+    rw ih g,
+    simp,
+  }
+end
+-/
+
+theorem length_list_nfresh (g : gensym α) (n : nat) : 
+  length (nfresh g n).1 = n :=
+begin
+  induction n with n ih generalizing g,
+  { simp [nfresh] },
+  { simp [nfresh_succ_eq_nfresh_fresh, ih] }
+end
+
+/- nfresh can be split across two calls -/
+theorem nfresh_concat (g : gensym α) {n m₁ m₂ : nat} :
+  n = m₁ + m₂ → (nfresh g n).2 = (nfresh (nfresh g m₁).2 m₂).2 :=
+begin
+  induction n with n ih generalizing m₁ m₂,
+  { intro h,
+    rw zero_left_of_add_zero h,
+    rw zero_right_of_add_zero h,
+    simp },
+  { cases m₂,
+    { simp, intro h, simp [h] },
+    { intro h,
+      rw nat.succ_eq_add_one at h,
+      rw nat.succ_eq_add_one at h,
+      rw ← add_assoc at h,
+      simp [ih (nat.succ.inj h),
+        nfresh_succ_gensym_eq_fresh_nfresh_gensym] } }
+end
+
+/-
+theorem nfresh_concat2 (g : gensym α) {n m₁ m₂ : nat} : n = m₁ + m₂ → 
+  (nfresh g n).1 = (nfresh g m₁).1 ++ (nfresh (nfresh g m₁).2 m₂).1 :=
+begin
+  induction n with n ih generalizing m₁ m₂,
+end
+-/
+
+def alt_nfresh (g : gensym α) : nat → (list α × gensym α)
+| 0       := ⟨[], g⟩
+| (n + 1) := ⟨map (λ i, g.f (g.offset + (i) * g.delta)) (range (n + 1)),
+             {offset := g.offset + (n + 1) * g.delta,
+              delta := g.delta,
+              f := g.f,
+              delta_pos := g.delta_pos,
+              f_inj := g.f_inj }⟩
+
+@[simp] theorem alt_zero (g : gensym α) : alt_nfresh g 0 = ⟨[], g⟩ := rfl
+
+@[simp] theorem alt_one (g : gensym α) : alt_nfresh g 1 = prod.map (λ a, [a]) id (fresh g) :=
+by simp [alt_nfresh, fresh, range, range_core]
+
+theorem alt_succ (g : gensym α) (n : nat) :
+  alt_nfresh g (n + 1) = ⟨(fresh g).1 :: (alt_nfresh (fresh g).2 n).1, (alt_nfresh (fresh g).2 n).2⟩ :=
+begin
+  induction n with n ih,
+  { simp },
+  {
+    simp [alt_nfresh, fresh],
+    split,
+    {
+      unfold range,
+      unfold range_core,
+
+    },
+    { rw nat.succ_eq_add_one, -- Algebra sucky
+      repeat { rw add_mul },
+      simp,
+      repeat { rw add_assoc },
+      rw ← add_assoc g.delta (n * g.delta) g.delta,
+      rw add_comm g.delta (n * g.delta),
+      rw add_assoc (n * g.delta) g.delta g.delta,
+      simp
+    }
+    
+  }
+end
+
+theorem alt_nfresh_eq_nfresh (g : gensym α) (n : nat) :
+  (nfresh g n).1 = (alt_nfresh g n).1 :=
+begin
+  induction n with n ih generalizing g,
+  { simp },
+  {
+
+  }
+end
+
+/-! # split -/
+
+/- Creates a set of n new gensym objects that are disjoint, in the sense that
+   they will not generate any equal terms in future fresh calls. -/
+def split (g : gensym α) : nat → list (gensym α)
+| 0       := []
+| (n + 1) := list.map (λ (e : (nat × gensym α)),
+           ⟨e.2.offset + (e.1 * e.2.delta), -- Add delta times the index
+            e.2.delta * (n + 1), -- Hilbert-hotel by the input number
+            e.2.f,
+            mul_pos e.2.delta_pos n.succ_pos,
+            e.2.f_inj⟩)
+            (enum (repeat g (n + 1)))
+
+@[simp] theorem split_zero (g : gensym α) : split g 0 = [] := rfl
+
+theorem length_split (g : gensym α) (n : nat) :
+  length (split g n) = n :=
+begin
+  cases n,
+  { simp },
+  { simp [split, length_enum, length_repeat] }
+end
+
+/-! # Uniqueness of fresh output -/
+
+/-! # descendant -/
+
+/- If a number of fresh calls can be made to get to a gensym from a first gensym,
+    then the second gensym is a descendant of the first -/
+-- NOTE: g₂ is a descendant if it can be arrived at via some number of nfresh calls
+--       AND g₂'s delta is divided by g₁'s (i.e. a product of some number of split calls)
+def descendant (g₁ g₂ : gensym α) := 
+  g₁.delta ∣ g₂.delta ∧ ∃ (n : nat), g₂ ≃ (nfresh g₁ n).2
+
+notation g₁ ` ↦ ` g₂ := descendant g₁ g₂
+
+@[refl] theorem descendant.refl (g : gensym α) : g ↦ g :=
+and.intro dvd_rfl (exists.intro 0 (by refl))
+
+@[trans] theorem descendant.trans {g₁ g₂ g₃ : gensym α} :
+  (g₁ ↦ g₂) → (g₂ ↦ g₃) → (g₁ ↦ g₃) :=
+begin
+  rintros ⟨hd1, n, ho1, hf1⟩ ⟨hd2, m, ho2, hf2⟩,
+  split,
+  { exact dvd_trans hd1 hd2 },
+  { rcases hd1 with ⟨k1, hk1⟩,
+    rw nfresh_offset at ho1,
+    rw nfresh_offset at ho2,
+    use k1 * m + n,
+    split,
+    { rw nfresh_offset,
+      simp [ho2, ho1, hk1, ← add_assoc, mul_add, mul_assoc] },
+    { rw nfresh_f at hf1,
+      rw nfresh_f at hf2,
+      simp [nfresh_f, hf1, hf2] } }
+end
+
+theorem descendant_init (g : gensym α) : init g.f_inj ↦ g :=
+begin
+  unfold init,
+  split,
+  { exact one_dvd g.delta },
+  { use g.offset,
+    split,
+    { simp [nfresh_offset _ g.offset] },
+    { simp [nfresh_f] } }
+end
+
+theorem nfresh_descendant (g : gensym α) (n : nat) : g ↦ (nfresh g n).2 :=
+and.intro (by simp [nfresh_offset]) (exists.intro n (by refl))
+
+theorem split_descendant (g : gensym α) (n : nat) : ∀ g₂ ∈ split g n, g ↦ g₂ :=
+begin
+  cases n,
+  { simp },
+  { simp [split, -repeat_succ, -repeat],
+    rintros g₂ d x hx rfl,
+    unfold descendant,
+    have := mem_snd_map_of_mem hx,
+    rw enum_map_snd at this,
+    rw eq_of_mem_repeat this,
+    split,
+    { simp },
+    { use d,
+      split,
+      { simp [add_comm, mul_comm] },
+      { simp } } }
+end
+
+/-! # disjoint -/
+
+def disjoint (g₁ g₂ : gensym α) := 
+  ((g₁.delta ∣ g₂.delta) ∨ (g₂.delta ∣ g₁.delta)) ∧ (g₁.f = g₂.f) ∧ 
+  (∀ (n m : nat), ((nfresh g₁ n).2.offset ≠ (nfresh g₂ m).2.offset))
+
+theorem disjoint.antirefl (g : gensym α) : ¬(disjoint g g) :=
+begin
+  rintros ⟨_, _, h⟩,
+  have := h 0 0,
+  contradiction
+end
+
+theorem disjoint_comm {g₁ g₂ : gensym α} :
+  disjoint g₁ g₂ ↔ disjoint g₂ g₁ :=
+begin
+  split;
+  { rintros ⟨hor, hf, h⟩,
+    unfold disjoint,
+    split,
+    { exact or.comm.mp hor },
+    { split,
+      { exact hf.symm },
+      { intros n m,
+        exact ne.symm (h m n) } } }
+end
+
+theorem not_disjoint_of_descendant {g₁ g₂ : gensym α} :
+  (g₁ ↦ g₂) → ¬(disjoint g₁ g₂) :=
+begin
+  rintros ⟨_, n, hn⟩ ⟨_, _, h⟩,
+  rw equiv_comm at hn,
+  have := h n 0,
+  rw nfresh_zero at this,
+  unfold snd at this,
+  exact this (hn.1)
+end
+
+theorem not_descendant_of_disjoint {g₁ g₂ : gensym α} :
+  disjoint g₁ g₂ → ¬(g₁ ↦ g₂) ∧ ¬(g₂ ↦ g₁) :=
+begin
+  rintros ⟨_, hf, h⟩,
+  split,
+  { rintros ⟨_, n, hno, hnf⟩,
+    have := ne.symm (h n 0),
+    rw nfresh_zero at this,
+    unfold snd at this,
+    exact this hno },
+  { rintros ⟨_, m, hmo, hmf⟩,
+    have := h 0 m,
+    rw nfresh_zero at this,
+    unfold snd at this,
+    exact this hmo }
+end
+
+theorem disjoint_fresh_of_disjoint {g₁ g₂ : gensym α} :
+  disjoint g₁ g₂ → disjoint (fresh g₁).2 g₂ :=
+begin
+  rintros ⟨hor, hf, h⟩,
+  split,
+  { rw fresh_delta, exact hor },
+  { split, 
+    { rw fresh_f, exact hf },
+    { intros n m,
+      rw ← nfresh_succ_gensym_eq_nfresh_fresh_gensym,
+      exact h (n + 1) m } }
+end
+
+theorem disjoint_nfresh_of_disjoint {g₁ g₂ : gensym α} (n : nat) :
+  disjoint g₁ g₂ → disjoint (nfresh g₁ n).2 g₂ :=
+begin
+  rintros ⟨hor, hf, h⟩,
+  split,
+  { rw nfresh_delta, exact hor },
+  { split,
+    { rw nfresh_f, exact hf },
+    { intros x y,
+      have : n + x = n + x, from rfl,
+      rw ← nfresh_concat g₁ this,
+      exact h (n + x) y } }
+end
+
+theorem inter_nil_of_disjoint [decidable_eq α] {g₁ g₂ : gensym α} :
+  disjoint g₁ g₂ → ∀ (n m : nat), (nfresh g₁ n).1 ∩ (nfresh g₂ m).1 = [] :=
+begin
+  rintros ⟨hdiv, hf, ho⟩ n m,
+  induction n with n ih generalizing g₁,
+  { simp },
+  {
+    rw nfresh_succ_eq_nfresh_fresh,
+    unfold fst,
+    have hfreshdel : (fresh g₁).2.delta ∣ g₂.delta ∨ g₂.delta ∣ (fresh g₁).2.delta,
+    { rw fresh_delta, exact hdiv },
+    have hfreshf : (fresh g₁).2.f = g₂.f,
+    { rw fresh_f, exact hf },
+    have hfresho : ∀ (n m : nat),
+      (nfresh (fresh g₁).2 n).2.offset ≠ (nfresh g₂ m).2.offset,
+    { intros n m,
+      rw ← nfresh_succ_gensym_eq_nfresh_fresh_gensym,
+      exact ho (n + 1) m },
+    have ihred := ih hfreshdel hfreshf hfresho,
+    have : (fresh g₁).1 ∉ (nfresh g₂ m).1,
+    {
+
+    }
+  }
+end
+
+end gensym
