src/xor/tseitin_general.lean
@@ -1,0 +1,57 @@
+/-
+This file proves that the Tseitin encoding holds for general propositional formulas.
+
+Authors: Cayden Codel, Jeremy Avigad, Marijn Heule
+Carnegie Mellon University
+-/
+
+import cnf.assignment
+import cnf.literal
+import cnf.clause
+import cnf.cnf
+
+-- First try : a formula is a literal
+-- Or it is two formulas joined by a connector,
+--   the connector is a formula of left and right halves to bool on eval
+inductive form : Type
+| lit : literal → form
+| conn : form → form → (bool → bool → bool) → form
+
+namespace form 
+
+open literal
+open assignment
+open clause
+open cnf
+
+protected def eval (α : assignment) (to_cnf : form → cnf) : form → bool
+| (lit l) := literal.eval α l
+| (conn f₁ f₂ op) := op (cnf.eval α (to_cnf f₁)) (cnf.eval α (to_cnf f₂))
+
+theorem tseitin_thm (α : assignment) (to_cnf : form → cnf) (f₁ f₂ : form) (op : bool → bool → bool) :
+  ∃ (α₂ : assignment), eqod α α₂ (cnf.vars (to_cnf f₁) ∪ cnf.vars (to_cnf f₂)) → 
+  ∃ (n : nat), n ∉ cnf.vars (to_cnf f₁) ∧ n ∉ cnf.vars (to_cnf f₂) →
+    cnf.eval α₂ (to_cnf (conn f₁ f₂ op)) = 
+      (band (cnf.eval α (to_cnf (conn f₁ (lit (Neg n)) bxor))) 
+            (cnf.eval α (to_cnf (conn (lit (Pos n)) f₂ bxor)))) :=
+begin
+  have max1 : (max (max_nat (cnf.vars (to_cnf f₁))) (max_nat (cnf.vars (to_cnf f₂)))) + 1 > max_nat (cnf.vars (to_cnf f₁)),
+  { have : max_nat (cnf.vars (to_cnf f₁)) ≤ max (max_nat (cnf.vars (to_cnf f₁))) (max_nat (cnf.vars (to_cnf f₂))),
+      from le_max_left (max_nat (vars (to_cnf f₁))) (max_nat (vars (to_cnf f₂))),
+    exact nat.lt_succ_iff.mpr this },
+  have notmem1 := not_mem_of_gt_max_nat max1,
+
+  have max2 : (max (max_nat (cnf.vars (to_cnf f₁))) (max_nat (cnf.vars (to_cnf f₂)))) + 1 > max_nat (cnf.vars (to_cnf f₂)),
+  { have : max_nat (cnf.vars (to_cnf f₂)) ≤ max (max_nat (cnf.vars (to_cnf f₁))) (max_nat (cnf.vars (to_cnf f₂))),
+      from le_max_right (max_nat (vars (to_cnf f₁))) (max_nat (vars (to_cnf f₂))),
+    exact nat.lt_succ_iff.mpr this },
+  have notmem2 := not_mem_of_gt_max_nat max2,
+
+  have notmem12 : (max (max_nat (cnf.vars (to_cnf f₁))) (max_nat (cnf.vars (to_cnf f₂)))) + 1 ∉ (cnf.vars (to_cnf f₁)) ∪ (cnf.vars (to_cnf f₂)),
+    simp [not_or_distrib, notmem1, notmem2],
+  
+  have := exists_extended_assignment_of_assignment α notmem12,
+  
+end
+
+end form
