src/xor/xor_general.lean
@@ -1,0 +1,480 @@
+/-
+
+  This file concerns the definition and translation of XOR gates into CNF, and
+  proves that this translation is correct.
+
+  Variables are general.
+
+  Authors: Cayden Codel, Jeremy Avigad, Marijn Heule
+  Carnegie Mellon University
+
+-/
+
+import data.bool
+import data.list.basic
+
+import cnf.literal_general
+import cnf.clause_general
+import cnf.cnf_general
+import cnf.explode_general
+import basic
+
+universe u
+
+-- Represents the parametric type of the variable stored in the literal
+variables {V : Type u} [decidable_eq V] [inhabited V]
+
+/- An n-literal XOR gate is a list of those literals -/
+def xor_gate (V : Type u) := list (literal V)
+
+namespace xor_gate
+
+open list
+open literal
+open clause
+open cnf
+open explode
+
+instance : has_append (xor_gate V) := ⟨list.append⟩
+
+-- The conversion of the XOR gate to a clause is a nice way of sweeping
+-- uner the rug that the two definitions are actually identical
+-- TODO canonical way of saying we want the nil/empty clause?
+def to_clause (g : xor_gate V) : clause V :=
+  g.foldr (λ l c, l :: c) []
+
+-- Kinda cheesy
+lemma gate_eq_clause (g : xor_gate V) : g = g.to_clause :=
+by simp [to_clause]
+
+/- Evaluates the XOR gate under an assignment -/
+def eval (α : assignment V) (g : xor_gate V) : bool :=
+  g.foldr (λ l b, b ⊕ l.eval α) ff
+
+@[simp] theorem eval_nil (α : assignment V) : eval α [] = ff := rfl
+
+protected theorem eval_cons (α : assignment V) (l : literal V) (g : xor_gate V) : 
+  eval α (l :: g) = bxor (literal.eval α l) (eval α g) :=
+by simp [eval, foldr_cons, bool.bxor_comm]
+
+theorem eval_concat (α : assignment V) (g₁ g₂ : xor_gate V) : eval α (g₁ ++ g₂) = bxor (eval α g₁) (eval α g₂) :=
+begin
+  induction g₁ with l ls ih,
+  { simp },
+  { simp [xor_gate.eval_cons, ih] }
+end
+
+theorem eval_cons_conjunctive (α : assignment V) (l : literal V) (g : xor_gate V) : 
+  eval α (l :: g) = (literal.eval α l || eval α g) && (!(literal.eval α l) || !(eval α g)) :=
+by simp only [← bxor_conjunctive, xor_gate.eval_cons α l g]
+
+theorem eval_cons_disjunctive (α : assignment V) (l : literal V) (g : xor_gate V) :
+  eval α (l :: g) = (!(literal.eval α l) && eval α g) || (literal.eval α l && !(eval α g)) :=
+by simp only [← bxor_disjunctive, xor_gate.eval_cons α l g]
+
+/- Using a recursive evaluation function is sometimes more convenient -/
+def eval_rec (α : assignment V) : xor_gate V → bool
+| []        := ff
+| (l :: ls) := l.eval α ⊕ eval_rec ls
+
+/- To use the recursive definition, we need to prove that the two functions are equivalent -/
+theorem eval_and_eval_rec_equiv (α : assignment V) (g : xor_gate V) : 
+  eval α g = eval_rec α g :=
+begin
+  induction g with l ls ih,
+  { simp [eval_rec, eval] },
+  { simp [eval_rec, ih, xor_gate.eval_cons] },
+end
+
+/- The XOR gate evaluates to true if an odd number of literals evaluates to true -/
+theorem xor_odd_eval_tt (α : assignment V) (g : xor_gate V) : 
+  g.eval α = nat.bodd (g.countp (λ l, l.eval α = tt)) :=
+begin
+  induction g with l ls ih,
+  { simp },
+  { cases h : (l.eval α);
+    { simp [xor_gate.eval_cons, h, ih] } }
+end
+
+-- This is a shortcut of the above that uses gate.to_clause instead
+-- NOTE that the to_clause is essentially an identity operation, but if sets/permuations are
+-- used instead, the proof may grow more complex
+theorem xor_odd_eval_tt2 (α : assignment V) (g : xor_gate V) :
+  g.eval α = nat.bodd (g.to_clause.count_tt α) :=
+begin
+  induction g with l ls ih,
+  { simp [to_clause] },
+  { cases h : (l.eval α);
+    { rw ← gate_eq_clause ls at ih,
+      simp [to_clause, xor_gate.eval_cons, count_tt_cons, bool.to_nat, h, ih] } }
+end
+
+/-! ## Naive encoding, simple version -/
+
+-- The naive encoding returns a formula with all possible clauses with an even number of negated literals
+-- Because we are using natural numbers, i.e. positive literals, we want an even number of negative literals
+def to_xor_cnf : list V → cnf V
+| []        := [[]]
+| (v :: vs) := (explode vs).map (λ c, cond (nat.bodd c.count_neg = ff) ((Pos v) :: c) ((Neg v) :: c))
+
+@[simp] theorem to_xor_cnf_nil : to_xor_cnf ([] : list V) = [[]] := rfl
+
+theorem mem_explode_of_mem_to_xor :
+  ∀ {l : list V}, ∀ {c : clause V}, c ∈ to_xor_cnf l → c ∈ explode l
+| []        := by simp [to_xor_cnf]
+| (v :: vs) := begin
+  simp [to_xor_cnf, mem_map, mem_append],
+  intros c hc,
+  have : (Pos v).var = v ∧ (Neg v).var = v, simp [var], -- Make into literal lemma?
+  cases h : (c.count_neg.bodd);
+  { simp [h, this],
+    apply mem_explode_cons_of_mem_explode_of_lit,
+    exact hc }
+end
+
+theorem length_to_xor_cnf : 
+  ∀ {l : list V}, l ≠ [] → length (to_xor_cnf l) = 2^(length l - 1)
+| []        := by { contradiction }
+| (n :: ns) := by simp [to_xor_cnf, length_explode]
+
+theorem length_to_xor_cnf_pos : ∀ {l : list V}, length (to_xor_cnf l) > 0
+| []        := by { simp [to_xor_cnf] }
+| (n :: ns) := by simp [length_to_xor_cnf]
+
+theorem exists_mem_to_xor_cnf : ∀ (l : list V),
+  ∃ (c : clause V), c ∈ to_xor_cnf l
+| [] := by simp [to_xor_cnf]
+| (v :: vs) := exists_mem_of_length_pos length_to_xor_cnf_pos
+
+theorem map_var_eq_of_mem_to_xor : 
+  ∀ {l : list V}, ∀ {c : clause V}, c ∈ to_xor_cnf l → c.map var = l
+| []        := by simp [to_xor_cnf]
+| (n :: ns) := begin
+  simp [to_xor_cnf],
+  intros c hc,
+  cases h : c.count_neg.bodd;
+  { simp [h, var, map_var_eq_of_mem_explode hc] }
+end
+
+theorem mem_to_xor_of_even_negation_of_map_var_eq : 
+  ∀ {l : list V}, ∀ {c : clause V}, c.map var = l → (nat.bodd c.count_neg = ff) → c ∈ to_xor_cnf l
+| []        := by simp [to_xor_cnf]
+| (n :: ns) := begin
+  intros c hc,
+  rcases exists_cons_of_map_cons hc with ⟨l, ls, rfl, hl, hls⟩,
+  rcases pos_or_neg_of_var_eq_nat hl with rfl | rfl;
+  { simp [count_neg_cons, is_neg, bool.to_nat, to_xor_cnf],
+    intro hcount, use ls,
+    simp [hcount, mem_explode_of_map_var_eq hls] }
+end
+
+theorem even_negation_of_mem_to_xor_of_map_var_eq : 
+  ∀ {l : list V}, ∀ {c : clause V}, c.map var = l → c ∈ to_xor_cnf l → nat.bodd c.count_neg = ff
+| []        := by simp
+| (n :: ns) := begin
+  intros c hc hxor,
+  simp [to_xor_cnf] at hxor,
+  rcases hxor with ⟨a, ha, hacons⟩,
+  rcases exists_cons_of_map_cons hc with ⟨l, ls, rfl, hl, hls⟩,
+  cases h : a.count_neg.bodd;
+  { simp [h] at hacons,
+    simp [← hacons, count_neg_cons, is_neg, bool.to_nat, h] },
+end
+
+theorem even_negation_iff_mem_to_xor 
+  {l : list V} {c : clause V} (hc : c.map var = l) : c ∈ to_xor_cnf l ↔ nat.bodd c.count_neg = ff :=
+⟨even_negation_of_mem_to_xor_of_map_var_eq hc,
+  mem_to_xor_of_even_negation_of_map_var_eq hc⟩
+
+theorem not_mem_to_xor_cnf_of_odd_negation_of_map_var_eq 
+  {l : list V} {c : clause V} : c.map var = l → (nat.bodd c.count_neg = tt) → c ∉ to_xor_cnf l :=
+begin
+  intros hc hcount,
+  by_contradiction,
+  exact absurd_bool hcount (even_negation_of_mem_to_xor_of_map_var_eq hc h)
+end
+
+-- TODO move the c.map var assumption into the ns list nat portion since the above need it too
+theorem odd_negation_of_not_mem_nat_to_xor_of_map_var_eq 
+  {l : list V} {c : clause V} (hc : c.map var = l) : c ∉ to_xor_cnf l → nat.bodd c.count_neg = tt :=
+begin
+  contrapose,
+  simp,
+  exact (even_negation_iff_mem_to_xor hc).mpr
+end
+
+theorem odd_negation_iff_not_mem_to_xor 
+  {l : list V} {c : clause V} (hc : c.map var = l) : c ∉ to_xor_cnf l ↔ nat.bodd c.count_neg = tt :=
+⟨odd_negation_of_not_mem_nat_to_xor_of_map_var_eq hc, 
+  not_mem_to_xor_cnf_of_odd_negation_of_map_var_eq hc⟩
+
+-- We prove that the naive encoding is equivalent to an XOR gate of all positive literals
+lemma exists_to_xor_cnf_of_xor {l : list V} 
+  : (∃ (α : assignment V), eval α (map Pos l) = tt) → 
+     ∃ (α₂ : assignment V), cnf.eval α₂ (to_xor_cnf l) = tt :=
+begin
+  rintros ⟨α, ha⟩,
+  rw xor_odd_eval_tt2 α (map Pos l) at ha,
+  rw ← gate_eq_clause (map Pos l) at ha,
+  use α,
+  apply eval_tt_iff_forall_clause_eval_tt.mpr,
+  intros c hc,
+  have mve := map_var_eq_of_mem_to_xor hc,
+  have neq := neq_of_ff_of_tt ha ((even_negation_iff_mem_to_xor mve).mp hc),
+  exact eval_tt_of_opposite_parity mve neq
+end
+
+lemma exists_xor_of_to_xor_cnf {l : list V}
+  : (∃ (α : assignment V), cnf.eval α (to_xor_cnf l) = tt) → 
+    ∃ (α₂ : assignment V), eval α₂ (map Pos l) = tt :=
+begin
+  rintros ⟨α, ha⟩,
+  use α,
+  rw xor_odd_eval_tt2 α (map Pos l),
+  rw ← gate_eq_clause (map Pos l),
+  rcases exists_mem_to_xor_cnf l with ⟨c, hc⟩,
+  have := eval_tt_iff_forall_clause_eval_tt.mp ha,
+  by_contradiction,
+  simp at h,
+  rw count_tt_pos_eq_count_neg_falsify at h,
+  have falsify_mem := mem_to_xor_of_even_negation_of_map_var_eq 
+    (map_var_falsify_eq_list α l) h,
+  have falsify_eval := falsify_eval_ff α l,
+  have := this (falsify α l) falsify_mem,
+  exact absurd_bool this falsify_eval
+end
+
+theorem equisatisfiable_to_xor_cnf (l : list V) :
+  assignment.equisatisfiable (λ α, cnf.eval α (to_xor_cnf l)) (λ α, xor_gate.eval α (map Pos l)) :=
+begin
+  split,
+  { rintros ⟨a, ha⟩,
+    simp at ha,
+    have : ∃ α, cnf.eval α (to_xor_cnf l) = tt,
+    { use [a, ha] },
+    exact exists_xor_of_to_xor_cnf this },
+  { rintros ⟨a, ha⟩,
+    simp at ha,
+    have : ∃ α, xor_gate.eval α (map Pos l) = tt,
+    {use [a, ha] },
+    exact exists_to_xor_cnf_of_xor this }
+end
+
+/-! # More complex encoding -/
+
+/-
+The above encoding assumed that the list of interest were only positive literals.
+Here, we generalize and prove the encoding valid with general lists of literals.
+The encoding is generated by counting "flips" between clauses rather than negations of literals.
+-/
+def xor_cnf : list (literal V) → cnf V
+| []        := [[]]
+| (l :: ls) := (explode (map var ls)).map (λ c, cond (nat.bodd (c.count_flips (ls)) = ff) (l :: c) (l.flip :: c))
+
+@[simp] theorem xor_cnf_nil : xor_cnf ([] : list (literal V)) = [[]] := rfl
+
+@[simp] theorem xor_cnf_singleton (l : literal V) : xor_cnf [l] = [[l]] :=
+by simp [xor_cnf]
+
+theorem mem_explode_of_mem_xor_cnf : ∀ {l : list (literal V)} {c : clause V}, 
+  c ∈ xor_cnf l → c ∈ explode (map var l)
+| []        := by simp [xor_cnf]
+| (l :: ls) := begin
+  simp [xor_cnf, explode],
+  intros c hc,
+  cases l,
+  { cases h : (nat.bodd (c.count_flips ls)),
+    { use c, simp [h, hc, var, literal.flip] },
+    { right, use c, simp [h, hc, var, literal.flip] } },
+  { cases h : (nat.bodd (c.count_flips ls)), 
+    { right, use c, simp [h, hc, var, literal.flip] },
+    { use c, simp [h, hc, var, literal.flip] } }
+end
+
+theorem length_xor_cnf : ∀ {l : list (literal V)}, 
+  l ≠ [] → length (xor_cnf l) = 2^(length l - 1)
+| []        := by { contradiction }
+| (l :: ls) := by simp [xor_cnf, length_explode]
+
+theorem length_xor_cnf_pos : ∀ {l : list (literal V)}, length (xor_cnf l) > 0
+| []        := by { simp [xor_cnf] }
+| (l :: ls) := by simp [length_xor_cnf]
+
+theorem exists_mem_xor_cnf : ∀ (l : list (literal V)),
+  ∃ (c : clause V), c ∈ xor_cnf l
+| []        := by simp [xor_cnf]
+| (v :: vs) := exists_mem_of_length_pos length_xor_cnf_pos
+
+theorem map_var_eq_of_mem_xor_cnf {l : list (literal V)} : ∀ {c : clause V}, 
+  c ∈ xor_cnf l → map var c = map var l :=
+begin
+  induction l with v vs ih,
+  { simp [xor_cnf] },
+  { simp [xor_cnf],
+    intros c hc,
+    cases h : (nat.bodd (c.count_flips vs));
+    { simp [h, map_var_eq_of_mem_explode hc, flip_var_eq v] } }
+end
+
+-- TODO choose to add back in lemmas on flips for literal
+theorem mem_xor_cnf_of_even_flips_of_map_var_eq : ∀ {l : list (literal V)}, 
+  ∀ {c : clause V}, map var c = map var l → 
+  (nat.bodd (c.count_flips l) = ff) → c ∈ xor_cnf l
+| []        := by simp [xor_cnf]
+| (l :: ls) := begin
+  simp [xor_cnf, map_cons],
+  intros c hc hcount,
+  rcases exists_cons_of_map_cons hc with ⟨d, ds, rfl, hd, hds⟩,
+  use ds,
+  cases htf : (nat.bodd (count_flips ds ls)),
+  { by_cases l.flip = d,
+    { have : d.flip = l, from congr_arg literal.flip h ▸ flip_flip l,
+      simp [count_flips, this] at hcount,
+      exact absurd_bool hcount htf },
+    { simp [htf, mem_explode_of_map_var_eq hds, hd],
+      rcases eq_or_flip_eq_of_var_eq hd with rfl | h₂,
+      { refl },
+      { have : d = l.flip, from congr_arg literal.flip h₂ ▸ (flip_flip d).symm, 
+        exact absurd this (ne.symm h) } } },
+  { by_cases l.flip = d,
+    { simp [htf, mem_explode_of_map_var_eq hds, hd, h], },
+    { have := function.injective.ne flip_injective h,
+      rw flip_flip at this,
+      simp [count_flips, ne.symm this] at hcount,
+      exact absurd_bool htf hcount } }
+end
+
+theorem even_flips_of_mem_xor_cnf_of_map_var_eq : ∀ {l : list (literal V)}, 
+  ∀ {c : clause V}, c.map var = map var l → 
+  c ∈ xor_cnf l → nat.bodd (count_flips c l) = ff
+| []        := by simp [xor_cnf]
+| (l :: ls) := begin
+  intros c hc hxor,
+  simp [xor_cnf] at hxor,
+  rcases hxor with ⟨a, ha, hacons⟩,
+  rcases exists_cons_of_map_cons hc with ⟨c, cs, rfl, hc2, hcs⟩,
+  cases h : (nat.bodd (count_flips a ls));
+  { simp [h] at hacons,
+    simp [← hacons, count_flips, is_neg, bool.to_nat, h, flip_flip _, flip_ne] }
+end
+
+theorem even_flips_iff_mem_xor_cnf {l : list (literal V)} {c : clause V} 
+  (hc : c.map var = map var l) :
+  nat.bodd (count_flips c l) = ff ↔ c ∈ xor_cnf l :=
+⟨mem_xor_cnf_of_even_flips_of_map_var_eq hc, even_flips_of_mem_xor_cnf_of_map_var_eq hc⟩
+
+theorem not_mem_xor_cnf_of_odd_flips_of_map_var_eq {l : list (literal V)} 
+  {c : clause V} : map var c = map var l → 
+  (nat.bodd (count_flips c l)) = tt → c ∉ xor_cnf l :=
+begin
+  intros hc hcount,
+  by_contradiction,
+  exact absurd_bool hcount ((even_flips_iff_mem_xor_cnf hc).mpr h)
+end
+
+theorem odd_flips_of_not_mem_xor_cnf_of_map_var_eq {l : list (literal V)} 
+  {c : clause V} : map var c = map var l → 
+  c ∉ xor_cnf l → (nat.bodd (count_flips c l)) = tt :=
+begin
+  intro hc,
+  contrapose,
+  simp,
+  exact (even_flips_iff_mem_xor_cnf hc).mp
+end
+
+theorem odd_flips_iff_not_mem_xor_cnf {l : list (literal V)} 
+  {c : clause V} (hc : map var c = map var l) :
+  nat.bodd (count_flips c l) = tt ↔ c ∉ xor_cnf l :=
+⟨not_mem_xor_cnf_of_odd_flips_of_map_var_eq hc, odd_flips_of_not_mem_xor_cnf_of_map_var_eq hc⟩
+
+lemma exists_xor_cnf_of_xor {l : list (literal V)} :
+  (∃ (α : assignment V), eval α l = tt) → 
+  ∃ (α₂ : assignment V), cnf.eval α₂ (xor_cnf l) = tt :=
+begin
+  rintros ⟨α, ha⟩,
+  rw xor_odd_eval_tt2 α l at ha,
+  rw ← gate_eq_clause l at ha,
+  use α,
+  apply eval_tt_iff_forall_clause_eval_tt.mpr,
+  intros c hc,
+  have mve := map_var_eq_of_mem_xor_cnf hc,
+  have neqodd := neq_of_ff_of_tt ha ((even_flips_iff_mem_xor_cnf mve).mpr hc),
+  have neq := ne_of_apply_ne nat.bodd neqodd,
+  rw count_flips_comm at neq,
+  exact eval_tt_of_neq_flips c mve.symm neq
+end
+
+lemma exists_xor_of_xor_cnf {l : list (literal V)} :
+  (∃ (α : assignment V), cnf.eval α (xor_cnf l) = tt) →
+  ∃ (α₂ : assignment V), eval α₂ l = tt :=
+begin
+  rintros ⟨α, ha⟩,
+  use α,
+  rw xor_odd_eval_tt2 α l,
+  rw ← gate_eq_clause l,
+  rcases exists_mem_xor_cnf l with ⟨c, hc⟩,
+  have := eval_tt_iff_forall_clause_eval_tt.mp ha,
+  by_contradiction,
+  simp at h,
+  rw [← count_flips_falsify_eq_count_tt, count_flips_comm] at h,
+  have falsify_mem := mem_xor_cnf_of_even_flips_of_map_var_eq
+    (map_var_falsify_eq_list α (map var l)) h,
+  have falsify_eval := falsify_eval_ff α (map var l),
+  have := this (falsify α (map var l)) falsify_mem,
+  exact absurd_bool this falsify_eval
+end
+
+theorem equisatisfiable_xor_cnf (l : list (literal V)) :
+  assignment.equisatisfiable (λ α, cnf.eval α (xor_cnf l)) (λ α, xor_gate.eval α l) :=
+begin
+  split,
+  { rintros ⟨α, ha⟩,
+    simp at ha,
+    have : ∃ α, cnf.eval α (xor_cnf l) = tt,
+    { use [α, ha] },
+    exact exists_xor_of_xor_cnf this },
+  { rintros ⟨α, ha⟩,
+    simp at ha,
+    have : ∃ α, xor_gate.eval α l = tt,
+    { use [α, ha] },
+    exact exists_xor_cnf_of_xor this }
+end
+
+theorem vars_cnf_subset_xor {ls : list (literal V)} :
+  ls ≠ [] → cnf.vars (xor_cnf ls) ⊆ (map var ls) :=
+begin
+  intro h,
+  cases ls,
+  { contradiction },
+  { intros n hn,
+    rcases cnf.exists_mem_clause_of_mem_vars hn with ⟨c, hcnf, hc⟩,
+    simp [← map_var_eq_of_mem_xor_cnf hcnf, mem_vars_iff_mem_map_vars, hc] }
+end
+
+end xor_gate
+
+/-! # Equivalence on domain for this encoding -/
+
+namespace assignment
+
+open list
+open literal
+open clause
+open xor_gate
+
+theorem equiv_on_domain_for_xor {α₁ α₂ : assignment V} {ls : list (literal V)} :
+  (α₁ ≡[map var ls]≡ α₂) → eval α₁ ls = eval α₂ ls :=
+begin
+  induction ls with v vs ih,
+  { simp },
+  { intro h,
+    simp [h, xor_gate.eval_cons],
+    cases heval : literal.eval α₁ v;
+    { cases v;
+      { simp [literal.eval] at heval,
+        simp [var] at h,
+        rw h v (mem_cons_self v _) at heval,
+        simp [heval, ih (eqod_of_eqod_cons h), literal.eval] } } }
+end
+
+end assignment
